Split and deduplicate Coq code

ecoop17/dsubsup_total_rec.v
@@ -7,361 +7,12 @@
  t ::= x | { Type = T } | lambda x:T.t | t t | unpack(t) { x => t }
  *)
 
-Require Export SfLib.
-
-Require Export Arith.EqNat.
-Require Export Arith.Le.
 Require Import Coq.Program.Equality.
-Require Import Omega.
 
-(* ### Syntax ### *)
-
-Definition id := nat.
-
-(* term variables occurring in types *)
-Inductive var : Type :=
-| varF : id -> var (* free, in concrete environment *)
-| varH : id -> var (* free, in abstract environment  *)
-| varB : id -> var (* locally-bound variable *)
-.
-
-Inductive ty : Type :=
-| TTop : ty
-| TBot : ty
-(* (z: T) -> T^z *)
-| TAll : ty -> ty -> ty
-(* x.Type *)
-| TSel : var -> ty
-(* { Type: S..U } *)
-| TMem : ty(*S*) -> ty(*U*) -> ty
-| TBind  : ty -> ty (* Recursive binder: { z => T^z },
-                         where z is locally bound in T *)
-| TAnd : ty -> ty -> ty (* Intersection Type: T1 /\ T2 *)
-.
-
-Inductive tm : Type :=
-(* x -- free variable, matching concrete environment *)
-| tvar : id -> tm
-(* { Type = T } *)
-| ttyp : ty -> tm
-(* lambda x:T.t *)
-| tabs : ty -> tm -> tm
-(* t t *)
-| tapp : tm -> tm -> tm
-(* unpack(e) { x => ... } *)
-| tunpack : tm -> tm -> tm                       
-.
-
-Inductive vl : Type :=
-(* a closure for a lambda abstraction *)
-| vabs : list vl (*H*) -> ty -> tm -> vl
-(* a closure for a first-class type *)
-| vty : list vl (*H*) -> ty -> vl
-.
-
-Definition tenv := list ty. (* Gamma environment: static *)
-Definition venv := list vl. (* H environment: run-time *)
-
-
-(* ### Representation of Bindings ### *)
-
-(* An environment is a list of values, indexed by decrementing ids. *)
-
-Fixpoint indexr {X : Type} (n : id) (l : list X) : option X :=
-  match l with
-    | [] => None
-    | a :: l' =>
-      if (beq_nat n (length l')) then Some a else indexr n l'
-  end.
-
-Inductive closed: nat(*B*) -> nat(*H*) -> nat(*F*) -> ty -> Prop :=
-| cl_top: forall i j k,
-    closed i j k TTop
-| cl_bot: forall i j k,
-    closed i j k TBot
-| cl_all: forall i j k T1 T2,
-    closed i j k T1 ->
-    closed (S i) j k T2 ->
-    closed i j k (TAll T1 T2)
-| cl_sel: forall i j k x,
-    k > x ->
-    closed i j k (TSel (varF x))
-| cl_selh: forall i j k x,
-    j > x ->
-    closed i j k (TSel (varH x))
-| cl_selb: forall i j k x,
-    i > x ->
-    closed i j k (TSel (varB x))
-| cl_mem: forall i j k T1 T2,
-    closed i j k T1 ->
-    closed i j k T2 ->
-    closed i j k (TMem T1 T2)
-| cl_bind: forall i j k T,
-    closed (S i) j k T ->
-    closed i j k (TBind T)
-| cl_and: forall i j k T1 T2,
-    closed i j k T1 ->
-    closed i j k T2 ->
-    closed i j k (TAnd T1 T2)
-.
-
-(* open define a locally-nameless encoding wrt to TVarB type variables. *)
-(* substitute var u for all occurrences of (varB k) *)
-Fixpoint open_rec (k: nat) (u: var) (T: ty) { struct T }: ty :=
-  match T with
-    | TTop        => TTop
-    | TBot        => TBot
-    | TAll T1 T2  => TAll (open_rec k u T1) (open_rec (S k) u T2)
-    | TSel (varF x) => TSel (varF x)
-    | TSel (varH i) => TSel (varH i)
-    | TSel (varB i) => if beq_nat k i then TSel u else TSel (varB i)
-    | TMem T1 T2  => TMem (open_rec k u T1) (open_rec k u T2)
-    | TBind T => TBind (open_rec (S k) u T)
-    | TAnd T1 T2 => TAnd (open_rec k u T1) (open_rec k u T2)
-  end.
-
-Definition open u T := open_rec 0 u T.
-
-(* Locally-nameless encoding with respect to varH variables. *)
-Fixpoint subst (U : var) (T : ty) {struct T} : ty :=
-  match T with
-    | TTop         => TTop
-    | TBot         => TBot
-    | TAll T1 T2   => TAll (subst U T1) (subst U T2)
-    | TSel (varB i) => TSel (varB i)
-    | TSel (varF i) => TSel (varF i)
-    | TSel (varH i) => if beq_nat i 0 then TSel U else TSel (varH (i-1))
-    | TMem T1 T2     => TMem (subst U T1) (subst U T2)
-    | TBind T       => TBind (subst U T)
-    | TAnd T1 T2    => TAnd (subst U T1)(subst U T2)
-  end.
-
-Fixpoint nosubst (T : ty) {struct T} : Prop :=
-  match T with
-    | TTop         => True
-    | TBot         => True
-    | TAll T1 T2   => nosubst T1 /\ nosubst T2
-    | TSel (varB i) => True
-    | TSel (varF i) => True
-    | TSel (varH i) => i <> 0
-    | TMem T1 T2    => nosubst T1 /\ nosubst T2
-    | TBind T       => nosubst T
-    | TAnd T1 T2    => nosubst T1 /\ nosubst T2
-  end.
-
-(* ### Subtyping ### *)
-(*
-Note: In contrast to the rules on paper, the subtyping 
-relation has two environments instead of just one.
-(The same holds for the semantic types, val_type, below).
-This split into an abstract and a concrete environment
-was necessary in the D<: soundness development, but is 
-not required here. We just keep it for consistency with
-our earlier Coq files.
-
-The first env is for looking up varF variables.
-The first env matches the concrete runtime environment, and is
-extended during type assignment.
-The second env is for looking up varH variables.
-The second env matches the abstract runtime environment, and is
-extended during subtyping.
-*)
-Inductive stp: tenv -> tenv -> ty -> ty -> Prop :=
-| stp_top: forall G1 GH T1,
-    closed 0 (length GH) (length G1) T1 ->
-    stp G1 GH T1 TTop
-| stp_bot: forall G1 GH T2,
-    closed 0 (length GH) (length G1) T2 ->
-    stp G1 GH TBot T2
-| stp_mem: forall G1 GH S1 U1 S2 U2,
-    stp G1 GH U1 U2 ->
-    stp G1 GH S2 S1 ->
-    stp G1 GH (TMem S1 U1) (TMem S2 U2)
-| stp_sel1: forall G1 GH TX T2 x,
-    indexr x G1 = Some TX ->
-    closed 0 0 (length G1) TX ->
-    stp G1 GH TX (TMem TBot T2) ->
-    stp G1 GH (TSel (varF x)) T2
-| stp_sel2: forall G1 GH TX T1 x,
-    indexr x G1 = Some TX ->
-    closed 0 0 (length G1) TX ->
-    stp G1 GH TX (TMem T1 TTop) ->
-    stp G1 GH T1 (TSel (varF x)) 
-| stp_selx: forall G1 GH v x,
-    indexr x G1 = Some v ->
-    stp G1 GH (TSel (varF x)) (TSel (varF x))
-| stp_sela1: forall G1 GH TX T2 x,
-    indexr x GH = Some TX ->
-    closed 0 x (length G1) TX ->
-    stp G1 GH TX (TMem TBot T2) ->
-    stp G1 GH (TSel (varH x)) T2
-| stp_sela2: forall G1 GH TX T1 x,
-    indexr x GH = Some TX ->
-    closed 0 x (length G1) TX ->
-    stp G1 GH TX (TMem T1 TTop) ->
-    stp G1 GH T1 (TSel (varH x)) 
-| stp_selax: forall G1 GH v x,
-    indexr x GH = Some v  ->
-    stp G1 GH (TSel (varH x)) (TSel (varH x))
-
-(* stp for recursive types and intersection types *)
-| stp_bindx: forall GH G1 T1 T1' T2 T2',
-    stp G1 (T1'::GH) T1' T2' ->
-    T1' = (open (varH (length GH)) T1) ->
-    T2' = (open (varH (length GH)) T2) ->
-    closed 1 (length GH) (length G1) T1 ->
-    closed 1 (length GH) (length G1) T2 ->
-    stp G1 GH (TBind T1) (TBind T2)
-
-| stp_and11: forall GH G1 T1 T2 T,
-    stp G1 GH T1 T ->
-    closed 0 (length GH) (length G1) T2 ->
-    stp G1 GH (TAnd T1 T2) T
-
-| stp_and12: forall GH G1 T1 T2 T,
-    stp G1 GH T2 T ->
-    closed 0 (length GH) (length G1) T1 ->
-    stp G1 GH (TAnd T1 T2) T
-
-| stp_and2: forall GH G1 T1 T2 T,
-    stp G1 GH T T1 ->
-    stp G1 GH T T2 ->
-    stp G1 GH T (TAnd T1 T2)
-
-
-| stp_all: forall G1 GH T1 T2 T3 T4 x,
-    stp G1 GH T3 T1 ->
-    x = length GH ->
-    closed 1 (length GH) (length G1) T2 ->
-    closed 1 (length GH) (length G1) T4 ->
-    stp G1 (T3::GH) (open (varH x) T2) (open (varH x) T4) ->
-    stp G1 GH (TAll T1 T2) (TAll T3 T4)
-| stp_trans: forall G1 GH T1 T2 T3,
-    stp G1 GH T1 T2 ->
-    stp G1 GH T2 T3 ->
-    stp G1 GH T1 T3
-.
-
-(* ### Type Assignment ### *)
-Inductive has_type : tenv -> tm -> ty -> Prop :=
-| t_var: forall x env T1,
-           indexr x env = Some T1 ->
-           stp env [] T1 T1 ->
-           has_type env (tvar x) T1
-(* pack a recursive type  *)
-| t_var_pack : forall G1 x T1 T1',
-           (* has_type G1 (tvar x) T1' -> *)
-           indexr x G1 = Some (open (varF x) T1) ->            
-           T1' = (open (varF x) T1) ->
-           closed 1 0 (length G1) T1 ->
-           has_type G1 (tvar x) (TBind T1) 
-(* unpack a recursive type: unpack(x:{z=>T^z}) { x:T^x => ... }  *)                    
-| t_unpack: forall env x y T1 T1' T2,
-           has_type env x (TBind T1) ->
-           T1' = (open (varF (length env)) T1) ->
-           has_type (T1'::env) y T2 ->
-           closed 0 0 (length env) T2 ->
-           has_type env (tunpack x y) T2
-
-(* intersection typing *)
-| t_and : forall env x T1 T2,
-           has_type env (tvar x) T1 ->
-           has_type env (tvar x) T2 ->
-           has_type env (tvar x) (TAnd T1 T2)
-
-               
-| t_typ: forall env T1,
-           closed 0 0 (length env) T1 ->
-           has_type env (ttyp T1) (TMem T1 T1)
-               
-| t_app: forall env f x T1 T2,
-           has_type env f (TAll T1 T2) ->
-           has_type env x T1 ->
-           closed 0 0 (length env) T2 ->
-           has_type env (tapp f x) T2
-| t_dapp:forall env f x T1 T2 T,
-           has_type env f (TAll T1 T2) ->
-           has_type env (tvar x) T1 ->
-           T = open (varF x) T2 ->
-           closed 0 0 (length env) T ->
-           has_type env (tapp f (tvar x)) T
-| t_abs: forall env y T1 T2,
-           has_type (T1::env) y (open (varF (length env)) T2) ->
-           closed 0 0 (length env) (TAll T1 T2) ->
-           has_type env (tabs T1 y) (TAll T1 T2)
-| t_sub: forall env e T1 T2,
-           has_type env e T1 ->
-           stp env [] T1 T2 ->
-           has_type env e T2
-.
-
-
-
-(* ### Evaluation (Big-Step Semantics) ### *)
-
-(*
-None             means timeout
-Some None        means stuck
-Some (Some v))   means result v
-Could use do-notation to clean up syntax.
-*)
-
-Fixpoint teval(n: nat)(env: venv)(t: tm){struct n}: option (option vl) :=
-  match n with
-    | 0 => None
-    | S n =>
-      match t with
-        | tvar x       => Some (indexr x env)
-        | ttyp T       => Some (Some (vty env T))
-        | tabs T y     => Some (Some (vabs env T y))
-        | tapp ef ex   =>
-          match teval n env ex with
-            | None => None
-            | Some None => Some None
-            | Some (Some vx) =>
-              match teval n env ef with
-                | None => None
-                | Some None => Some None
-                | Some (Some (vty _ _)) => Some None
-                | Some (Some (vabs env2 _ ey)) =>
-                  teval n (vx::env2) ey
-              end
-          end
-        | tunpack ex ey =>
-          match teval n env ex with
-            | None => None
-            | Some None => Some None
-            | Some (Some vx) =>
-              teval n (vx::env) ey 
-          end
-      end
-  end.
-
-
-Definition tevaln env e v := exists nm, forall n, n > nm -> teval n env e = Some (Some v).
-
+Require Import dsubsup_total_rec_base.
+Require Import dsubsup_total_rec_binding.
 
 (* ### Semantic Interpretation of Types (Logical Relations) ### *)
-
-Fixpoint tsize_flat(T: ty) :=
-  match T with
-    | TTop => 1
-    | TBot => 1
-    | TAll T1 T2 => S (tsize_flat T1 + tsize_flat T2)
-    | TSel _ => 1
-    | TMem T1 T2 => S (tsize_flat T1 + tsize_flat T2)	
-    | TBind T => S (tsize_flat T)
-    | TAnd T1 T2 => S (tsize_flat T1 + tsize_flat T2)
-  end. 
-
-Lemma open_preserves_size: forall T x j,
-  tsize_flat T = tsize_flat (open_rec j (varH x) T).
-Proof.
-  intros T. induction T; intros; simpl; eauto.
-  - destruct v; simpl; destruct (beq_nat j i); eauto.
-Qed.
-
-
 (* NEW DESIGN IDEA:
   
    The required invariants about runtime evaluation rely in crucial
@@ -704,432 +355,6 @@ Qed.
 
 Hint Immediate wf_length.
 
-Lemma indexr_max : forall X vs n (T: X),
-                       indexr n vs = Some T ->
-                       n < length vs.
-Proof.
-  intros X vs. induction vs.
-  - Case "nil". intros. inversion H.
-  - Case "cons".
-    intros. inversion H.
-    case_eq (beq_nat n (length vs)); intros E2.
-    + SSCase "hit".
-      eapply beq_nat_true in E2. subst n. compute. eauto.
-    + SSCase "miss".
-      rewrite E2 in H1.
-      assert (n < length vs). eapply IHvs. apply H1.
-      compute. eauto.
-Qed.
-
-Lemma le_xx : forall a b,
-                       a <= b ->
-                       exists E, le_lt_dec a b = left E.
-Proof. intros.
-  case_eq (le_lt_dec a b). intros. eauto.
-  intros. omega.
-Qed.
-Lemma le_yy : forall a b,
-                       a > b ->
-                       exists E, le_lt_dec a b = right E.
-Proof. intros.
-  case_eq (le_lt_dec a b). intros. omega.
-  intros. eauto.
-Qed.
-
-Lemma indexr_extend : forall X vs n x (T: X),
-                       indexr n vs = Some T ->
-                       indexr n (x::vs) = Some T.
-
-Proof.
-  intros.
-  assert (n < length vs). eapply indexr_max. eauto.
-  assert (beq_nat n (length vs) = false) as E. eapply beq_nat_false_iff. omega.
-  unfold indexr. unfold indexr in H. rewrite H. rewrite E. reflexivity.
-Qed.
-
-(* splicing -- for stp_extend. *)
-
-Fixpoint splice n (T : ty) {struct T} : ty :=
-  match T with
-    | TTop         => TTop
-    | TBot         => TBot
-    | TAll T1 T2   => TAll (splice n T1) (splice n T2)
-    | TSel (varF i) => TSel (varF i)
-    | TSel (varB i) => TSel (varB i)
-    | TSel (varH i) => if le_lt_dec n i then TSel (varH (i+1)) else TSel (varH i)
-    | TMem T1 T2   => TMem (splice n T1) (splice n T2)
-    | TBind T      => TBind (splice n T)
-    | TAnd T1 T2   => TAnd (splice n T1) (splice n T2)
-  end.
-
-Definition spliceat n (V: (venv*ty)) :=
-  match V with
-    | (G,T) => (G,splice n T)
-  end.
-
-Lemma splice_open_permute: forall {X} (G0:list X) T2 n j,
-(open_rec j (varH (n + S (length G0))) (splice (length G0) T2)) =
-(splice (length G0) (open_rec j (varH (n + length G0)) T2)).
-Proof.
-  intros X G T. induction T; intros; simpl; eauto;
-  try rewrite IHT1; try rewrite IHT2; try rewrite IHT; eauto;
-  destruct v; eauto.
-
-  case_eq (le_lt_dec (length G) i); intros E LE; simpl; eauto.
-  rewrite LE. eauto.
-  rewrite LE. eauto.
-  case_eq (beq_nat j i); intros E; simpl; eauto.
-  case_eq (le_lt_dec (length G) (n + length G)); intros EL LE.
-  rewrite E.
-  assert (n + S (length G) = n + length G + 1). omega.
-  rewrite H. eauto.
-  omega.
-  rewrite E. eauto.
-Qed.
-
-Lemma indexr_splice_hi: forall G0 G2 x0 v1 T,
-    indexr x0 (G2 ++ G0) = Some T ->
-    length G0 <= x0 ->
-    indexr (x0 + 1) (map (splice (length G0)) G2 ++ v1 :: G0) = Some (splice (length G0) T).
-Proof.
-  intros G0 G2. induction G2; intros.
-  - eapply indexr_max in H. simpl in H. omega.
-  - simpl in H.
-    case_eq (beq_nat x0 (length (G2 ++ G0))); intros E.
-    + rewrite E in H. inversion H. subst. simpl.
-      rewrite app_length in E.
-      rewrite app_length. rewrite map_length. simpl.
-      assert (beq_nat (x0 + 1) (length G2 + S (length G0)) = true). {
-        eapply beq_nat_true_iff. eapply beq_nat_true_iff in E. omega.
-      }
-      rewrite H1. eauto.
-    + rewrite E in H.  eapply IHG2 in H. eapply indexr_extend. eapply H. eauto.
-Qed.
-
-Lemma indexr_spliceat_hi: forall G0 G2 x0 v1 G T,
-    indexr x0 (G2 ++ G0) = Some (G, T) ->
-    length G0 <= x0 ->
-    indexr (x0 + 1) (map (spliceat (length G0)) G2 ++ v1 :: G0) =
-    Some (G, splice (length G0) T).
-Proof.
-  intros G0 G2. induction G2; intros.
-  - eapply indexr_max in H. simpl in H. omega.
-  - simpl in H. destruct a.
-    case_eq (beq_nat x0 (length (G2 ++ G0))); intros E.
-    + rewrite E in H. inversion H. subst. simpl.
-      rewrite app_length in E.
-      rewrite app_length. rewrite map_length. simpl.
-      assert (beq_nat (x0 + 1) (length G2 + S (length G0)) = true). {
-        eapply beq_nat_true_iff. eapply beq_nat_true_iff in E. omega.
-      }
-      rewrite H1. eauto.
-    + rewrite E in H.  eapply IHG2 in H. eapply indexr_extend. eapply H. eauto.
-Qed.
-
-Lemma plus_lt_contra: forall a b,
-  a + b < b -> False.
-Proof.
-  intros a b H. induction a.
-  - simpl in H. apply lt_irrefl in H. assumption.
-  - simpl in H. apply IHa. omega.
-Qed.
-
-Lemma indexr_splice_lo0: forall {X} G0 G2 x0 (T:X),
-    indexr x0 (G2 ++ G0) = Some T ->
-    x0 < length G0 ->
-    indexr x0 G0 = Some T.
-Proof.
-  intros X G0 G2. induction G2; intros.
-  - simpl in H. apply H.
-  - simpl in H.
-    case_eq (beq_nat x0 (length (G2 ++ G0))); intros E.
-    + eapply beq_nat_true_iff in E. subst.
-      rewrite app_length in H0. apply plus_lt_contra in H0. inversion H0.
-    + rewrite E in H. apply IHG2. apply H. apply H0.
-Qed.
-
-Lemma indexr_extend_mult: forall {X} G0 G2 x0 (T:X),
-    indexr x0 G0 = Some T ->
-    indexr x0 (G2++G0) = Some T.
-Proof.
-  intros X G0 G2. induction G2; intros.
-  - simpl. assumption.
-  - simpl.
-    case_eq (beq_nat x0 (length (G2 ++ G0))); intros E.
-    + eapply beq_nat_true_iff in E.
-      apply indexr_max in H. subst.
-      rewrite app_length in H. apply plus_lt_contra in H. inversion H.
-    + apply IHG2. assumption.
-Qed.
-
-Lemma indexr_splice_lo: forall G0 G2 x0 v1 T f,
-    indexr x0 (G2 ++ G0) = Some T ->
-    x0 < length G0 ->
-    indexr x0 (map (splice f) G2 ++ v1 :: G0) = Some T.
-Proof.
-  intros.
-  assert (indexr x0 G0 = Some T). eapply indexr_splice_lo0; eauto.
-  eapply indexr_extend_mult. eapply indexr_extend. eauto.
-Qed.
-
-Lemma indexr_spliceat_lo: forall G0 G2 x0 v1 G T f,
-    indexr x0 (G2 ++ G0) = Some (G, T) ->
-    x0 < length G0 ->
-    indexr x0 (map (spliceat f) G2 ++ v1 :: G0) = Some (G, T).
-Proof.
-  intros.
-  assert (indexr x0 G0 = Some (G, T)). eapply indexr_splice_lo0; eauto.
-  eapply indexr_extend_mult. eapply indexr_extend. eauto.
-Qed.
-
-Lemma closed_splice: forall i j k T n,
-  closed i j k T ->
-  closed i (S j) k (splice n T).
-Proof.
-  intros. induction H; simpl; eauto.
-  case_eq (le_lt_dec n x); intros E LE.
-  apply cl_selh. omega.
-  apply cl_selh. omega.
-Qed.
-
-Lemma map_splice_length_inc: forall G0 G2 v1,
-   (length (map (splice (length G0)) G2 ++ v1 :: G0)) = (S (length (G2 ++ G0))).
-Proof.
-  intros. rewrite app_length. rewrite map_length. induction G2.
-  - simpl. reflexivity.
-  - simpl. eauto.
-Qed.
-
-Lemma map_spliceat_length_inc: forall G0 G2 v1,
-   (length (map (spliceat (length G0)) G2 ++ v1 :: G0)) = (S (length (G2 ++ G0))).
-Proof.
-  intros. rewrite app_length. rewrite map_length. induction G2.
-  - simpl. reflexivity.
-  - simpl. eauto.
-Qed.
-
-Lemma closed_inc_mult: forall i j k T,
-  closed i j k T ->
-  forall i' j' k',
-  i' >= i -> j' >= j -> k' >= k ->
-  closed i' j' k' T.
-Proof.
-  intros i j k T H. induction H; intros; eauto; try solve [constructor; omega].
-  - apply cl_all. apply IHclosed1; omega. apply IHclosed2; omega.
-  - constructor. apply IHclosed; omega.
-Qed.
-
-Lemma closed_inc: forall i j k T,
-  closed i j k T ->
-  closed i (S j) k T.
-Proof.
-  intros. apply (closed_inc_mult i j k T H i (S j) k); omega.
-Qed.
-
-Lemma closed_splice_idem: forall i j k T n,
-                            closed i j k T ->
-                            n >= j ->
-                            splice n T = T.
-Proof.
-  intros. induction H; eauto.
-  - (* TAll *) simpl.
-    rewrite IHclosed1. rewrite IHclosed2.
-    reflexivity.
-    assumption. assumption.
-  - (* TVarH *) simpl.
-    case_eq (le_lt_dec n x); intros E LE. omega. reflexivity.
-  - (* TMem *) simpl.
-    rewrite IHclosed1. rewrite IHclosed2.
-    reflexivity.
-    assumption. assumption.
-  - simpl. rewrite IHclosed. reflexivity. assumption.
-  - simpl. rewrite IHclosed1. rewrite IHclosed2. reflexivity. assumption. assumption.
-Qed.
-
-Lemma stp_closed : forall G GH T1 T2,
-                     stp G GH T1 T2 ->
-                     closed 0 (length GH) (length G) T1 /\ closed 0 (length GH) (length G) T2.
-Proof.
-  intros. induction H;
-    try solve [repeat ev; split; try inv_mem; eauto using indexr_max].
-Qed.
-
-Lemma stp_closed2 : forall G1 GH T1 T2,
-                       stp G1 GH T1 T2 ->
-                       closed 0 (length GH) (length G1) T2.
-Proof.
-  intros. apply (proj2 (stp_closed G1 GH T1 T2 H)).
-Qed.
-
-Lemma stp_closed1 : forall G1 GH T1 T2,
-                       stp G1 GH T1 T2 ->
-                       closed 0 (length GH) (length G1) T1.
-Proof.
-  intros. apply (proj1 (stp_closed G1 GH T1 T2 H)).
-Qed.
-
-
-Lemma closed_upgrade: forall i j k i' T,
- closed i j k T ->
- i' >= i ->
- closed i' j k T.
-Proof.
- intros. apply (closed_inc_mult i j k T H i' j k); omega.
-Qed.
-
-Lemma closed_upgrade_free: forall i j k j' T,
- closed i j k T ->
- j' >= j ->
- closed i j' k T.
-Proof.
- intros. apply (closed_inc_mult i j k T H i j' k); omega.
-Qed.
-
-Lemma closed_upgrade_freef: forall i j k k' T,
- closed i j k T ->
- k' >= k ->
- closed i j k' T.
-Proof.
- intros. apply (closed_inc_mult i j k T H i j k'); omega.
-Qed.
-
-Lemma closed_open: forall i j k V T, closed (i+1) j k T -> closed i j k (TSel V) ->
-  closed i j k (open_rec i V T).
-Proof.
-  intros. generalize dependent i.
-  induction T; intros; inversion H;
-  try econstructor;
-  try eapply IHT1; eauto; try eapply IHT2; eauto; try eapply IHT; eauto.
-  eapply closed_upgrade. eauto. eauto.
-  - Case "TVarB". simpl.
-    case_eq (beq_nat i x); intros E. eauto.
-    econstructor. eapply beq_nat_false_iff in E. omega.
-  - eapply closed_upgrade. eassumption. omega.
-Qed.
-
-Lemma indexr_has: forall X (G: list X) x,
-  length G > x ->
-  exists v, indexr x G = Some v.
-Proof.
-  intros. remember (length G) as n.
-  generalize dependent x.
-  generalize dependent G.
-  induction n; intros; try omega.
-  destruct G; simpl.
-  - simpl in Heqn. inversion Heqn.
-  - simpl in Heqn. inversion Heqn. subst.
-    case_eq (beq_nat x (length G)); intros E.
-    + eexists. reflexivity.
-    + apply beq_nat_false in E. apply IHn; eauto.
-      omega.
-Qed.
-
-Lemma stp_refl_aux: forall n T G GH,
-  closed 0 (length GH) (length G) T ->
-  tsize_flat T < n ->
-  stp G GH T T.
-Proof.
-  intros n. induction n; intros; try omega.
-  inversion H; subst; eauto;
-  try solve [omega];
-  try solve [simpl in H0; constructor; apply IHn; eauto; try omega];
-  try solve [apply indexr_has in H1; destruct H1; eauto].
-  - simpl in H0.
-    eapply stp_all.
-    eapply IHn; eauto; try omega.
-    reflexivity.
-    assumption.
-    assumption.
-    apply IHn; eauto.
-    simpl. apply closed_open; auto using closed_inc.
-    unfold open. rewrite <- open_preserves_size. omega.
-  - remember (open (varH (length GH)) T0) as TT.
-    assert (stp G (TT :: GH) TT TT). eapply IHn. subst.
-    eapply closed_open. simpl. eapply closed_upgrade_free. eassumption. omega.
-    constructor. simpl. omega. subst. unfold open. erewrite <- open_preserves_size. simpl in H0. omega.
-    eapply stp_bindx; try eassumption.
-  - simpl in *. assert (stp G GH T1 T1). eapply IHn; try eassumption; try omega.
-    assert (stp G GH T2 T2). eapply IHn; try eassumption; try omega.
-    eapply stp_and2; try eassumption. econstructor; try eassumption. eapply stp_and12; try eassumption.
-Qed.
-
-Lemma stp_refl: forall T G GH,
-  closed 0 (length GH) (length G) T ->
-  stp G GH T T.
-Proof.
-  intros. apply stp_refl_aux with (n:=S (tsize_flat T)); eauto.
-Qed.
-
-
-Lemma concat_same_length: forall {X} (GU: list X) (GL: list X) (GH1: list X) (GH0: list X),
-  GU ++ GL = GH1 ++ GH0 ->
-  length GU = length GH1 ->
-  GU=GH1 /\ GL=GH0.
-Proof.
-  intros. generalize dependent GH1. induction GU; intros.
-  - simpl in H0. induction GH1. rewrite app_nil_l in H. rewrite app_nil_l in H.
-    split. reflexivity. apply H.
-    simpl in H0. omega.
-  - simpl in H0. induction GH1. simpl in H0. omega.
-    simpl in H0. inversion H0. simpl in H. inversion H. specialize (IHGU GH1 H4 H2).
-    destruct IHGU. subst. split; reflexivity.
-Qed.
-
-Lemma concat_same_length': forall {X} (GU: list X) (GL: list X) (GH1: list X) (GH0: list X),
-  GU ++ GL = GH1 ++ GH0 ->
-  length GL = length GH0 ->
-  GU=GH1 /\ GL=GH0.
-Proof.
-  intros.
-  assert (length (GU ++ GL) = length (GH1 ++ GH0)) as A. {
-    rewrite H. reflexivity.
-  }
-  rewrite app_length in A. rewrite app_length in A.
-  rewrite H0 in A. apply Nat.add_cancel_r in A.
-  apply concat_same_length; assumption.
-Qed.
-
-
-Lemma indexr_at_index: forall {A} x0 GH0 GH1 (v:A),
-  beq_nat x0 (length GH1) = true ->
-  indexr x0 (GH0 ++ v :: GH1) = Some v.
-Proof.
-  intros. apply beq_nat_true in H. subst.
-  induction GH0.
-  - simpl. rewrite <- beq_nat_refl. reflexivity.
-  - simpl.
-    rewrite app_length. simpl. rewrite <- plus_n_Sm. rewrite <- plus_Sn_m.
-    rewrite false_beq_nat. assumption. omega.
-Qed.
-
-Lemma indexr_same: forall {A} x0 (v0:A) GH0 GH1 (v:A) (v':A),
-  beq_nat x0 (length GH1) = false ->
-  indexr x0 (GH0 ++ v :: GH1) = Some v0 ->
-  indexr x0 (GH0 ++ v' :: GH1) = Some v0.
-Proof.
-  intros ? ? ? ? ? ? ? E H.
-  induction GH0.
-  - simpl. rewrite E. simpl in H. rewrite E in H. apply H.
-  - simpl.
-    rewrite app_length. simpl.
-    case_eq (beq_nat x0 (length GH0 + S (length GH1))); intros E'.
-    simpl in H. rewrite app_length in H. simpl in H. rewrite E' in H.
-    rewrite H. reflexivity.
-    simpl in H. rewrite app_length in H. simpl in H. rewrite E' in H.
-    rewrite IHGH0. reflexivity. assumption.
-Qed.
-
-Inductive venv_ext : venv -> venv -> Prop :=
-| venv_ext_refl : forall G, venv_ext G G
-| venv_ext_cons : forall T G1 G2, venv_ext G1 G2 -> venv_ext (T::G1) G2.
-
-Lemma venv_ext__ge_length:
-  forall G G',
-    venv_ext G' G ->
-    length G' >= length G.
-Proof.
-  intros. induction H; simpl; omega.
-Qed.
 
 
 Lemma indexr_safe_ex: forall H1 GH G1 TF i,
@@ -1142,211 +367,6 @@ Proof.
 Qed.
 
 
-(* ### Substitution for relating static and dynamic semantics ### *)
-Lemma indexr_hit2 {X}: forall x (B:X) A G,
-  length G = x ->
-  B = A ->
-  indexr x (B::G) = Some A.
-Proof.
-  intros.
-  unfold indexr.
-  assert (beq_nat x (length G) = true). eapply beq_nat_true_iff. eauto.
-  rewrite H1. subst. reflexivity.
-Qed.
-
-Lemma indexr_miss {X}: forall x (B:X) A G,
-  indexr x (B::G) = A ->
-  x <> (length G)  ->
-  indexr x G = A.
-Proof.
-  intros.
-  unfold indexr in H.
-  assert (beq_nat x (length G) = false). eapply beq_nat_false_iff. eauto.
-  rewrite H1 in H. eauto.
-Qed.
-
-Lemma indexr_hit {X}: forall x (B:X) A G,
-  indexr x (B::G) = Some A ->
-  x = length G ->
-  B = A.
-Proof.
-  intros.
-  unfold indexr in H.
-  assert (beq_nat x (length G) = true). eapply beq_nat_true_iff. eauto.
-  rewrite H1 in H. inversion H. eauto.
-Qed.
-
-Lemma indexr_hit0: forall GH (GX0:venv) (TX0:ty),
-      indexr 0 (GH ++ [(GX0, TX0)]) =
-      Some (GX0, TX0).
-Proof.
-  intros GH. induction GH.
-  - intros. simpl. eauto.
-  - intros. simpl. destruct a. simpl. rewrite app_length. simpl.
-    assert (length GH + 1 = S (length GH)). omega. rewrite H.
-    eauto.
-Qed.
-
-Hint Resolve beq_nat_true_iff.
-Hint Resolve beq_nat_false_iff.
-
-Lemma closed_no_open: forall T x i j k,
-  closed i j k T ->
-  T = open_rec i x T.
-Proof.
-  intros. induction H; intros; eauto;
-  try solve [compute; compute in IHclosed; rewrite <-IHclosed; auto];
-  try solve [compute; compute in IHclosed1; compute in IHclosed2;
-             rewrite <-IHclosed1; rewrite <-IHclosed2; auto].
-
-  Case "TVarB".
-    unfold open_rec. assert (i <> x0). omega.
-    apply beq_nat_false_iff in H0.
-    rewrite H0. auto.
-Qed.
-
-Lemma open_subst_commute: forall T2 V j k x i,
-closed i j k (TSel V) ->
-(open_rec i (varH x) (subst V T2)) =
-(subst V (open_rec i (varH (x+1)) T2)).
-Proof. 
-  intros T2 TX j k. induction T2; intros; eauto; try destruct v; eauto.
-  - simpl. rewrite IHT2_1; eauto. rewrite IHT2_2; eauto.
-    eapply closed_upgrade. eauto. eauto.
-  - simpl.
-    case_eq (beq_nat i 0); intros E.
-    apply beq_nat_true in E. subst.
-    case_eq (beq_nat i0 0); intros E0.
-    apply beq_nat_true in E0. subst.
-    destruct TX; eauto.
-    simpl. destruct i; eauto.
-    inversion H; subst. omega.
-    simpl. reflexivity.
-    case_eq (beq_nat i0 0); intros E0.
-    apply beq_nat_true in E0. subst.
-    simpl. destruct TX; eauto.
-    case_eq (beq_nat i i0); intros E1.
-    apply beq_nat_true in E1. subst.
-    inversion H; subst. omega.
-    reflexivity.
-    simpl. reflexivity.
-  - simpl.
-    case_eq (beq_nat i i0); intros E.
-    apply beq_nat_true in E; subst.
-    simpl.
-    assert (x+1 <> 0) as A by omega.
-    eapply beq_nat_false_iff in A.
-    rewrite A.
-    assert (x = x + 1 - 1) as B. unfold id. omega.
-    rewrite <- B. reflexivity.
-    simpl. reflexivity.
-  - simpl. rewrite IHT2_1. rewrite IHT2_2. eauto. eauto. eauto.
-  - simpl. rewrite IHT2. reflexivity. eapply closed_upgrade. eassumption. omega.
-  - simpl. rewrite IHT2_1. rewrite IHT2_2. reflexivity. assumption. assumption.
-Qed.
-
-Lemma closed_no_subst: forall T i k TX,
-   closed i 0 k T ->
-   subst TX T = T.
-Proof.
-  intros T. induction T; intros; inversion H; simpl; eauto;
-  try solve [rewrite (IHT i k TX); eauto; try omega];
-  try solve [rewrite (IHT1 i k TX); eauto; rewrite (IHT2 (S i) k TX); eauto; try omega];
-  try solve [rewrite (IHT1 i k TX); eauto; rewrite (IHT2 i k TX); eauto; try omega];
-  try omega.
-  erewrite IHT. reflexivity. eassumption.
-Qed.
-
-Lemma closed_subst: forall i j k V T, closed i (j+1) k T -> closed 0 j k (TSel V) -> closed i j k (subst V T).
-Proof.
-  intros. generalize dependent i.
-  induction T; intros; inversion H;
-  try econstructor;
-  try eapply IHT1; eauto; try eapply IHT2; eauto; try eapply IHT; eauto.
-
-  - Case "TVarH". simpl.
-    case_eq (beq_nat x 0); intros E.
-    eapply closed_upgrade. eapply closed_upgrade_free.
-    eauto. omega. eauto. omega.
-    econstructor. assert (x > 0). eapply beq_nat_false_iff in E. omega. omega.
-Qed.
-
-Lemma closed_nosubst: forall i j k V T, closed i (j+1) k T -> nosubst T -> closed i j k (subst V T).
-Proof.
-  intros. generalize dependent i.
-  induction T; intros; inversion H;
-  try econstructor;
-  try eapply IHT1; eauto; try eapply IHT2; eauto; try eapply IHT; eauto; subst;
-  try inversion H0; eauto.
-
-  - Case "TVarH". simpl. simpl in H0. unfold id in H0.
-    assert (beq_nat x 0 = false) as E. apply beq_nat_false_iff. assumption.
-    rewrite E.
-    eapply cl_selh. omega.
-Qed.
-
-Lemma subst_open_commute_m: forall i j k k' j' V T2, closed (i+1) (j+1) k T2 -> closed 0 j' k' (TSel V) ->
-    subst V (open_rec i (varH (j+1)) T2) = open_rec i (varH j) (subst V T2).
-Proof.
-  intros.
-  generalize dependent i. generalize dependent j.
-  induction T2; intros; inversion H; simpl; eauto; subst;
-  try rewrite IHT2_1;
-  try rewrite IHT2_2;
-  try rewrite IHT2; eauto.
-  - Case "TVarH". simpl. case_eq (beq_nat x 0); intros E.
-    eapply closed_no_open. eapply closed_upgrade. eauto. omega.
-    eauto.
-  - Case "TVarB". simpl. case_eq (beq_nat i x); intros E.
-    simpl. case_eq (beq_nat (j+1) 0); intros E2.
-    eapply beq_nat_true_iff in E2. omega.
-    subst. assert (j+1-1 = j) as A. omega. rewrite A. eauto.
-    eauto.
-Qed.
-
-Lemma subst_open_commute: forall i j k k' V T2, closed (i+1) (j+1) k T2 -> closed 0 0 k' (TSel V) ->
-    subst V (open_rec i (varH (j+1)) T2) = open_rec i (varH j) (subst V T2).
-Proof.
-  intros. eapply subst_open_commute_m; eauto.
-Qed.
-
-Lemma subst_open_zero: forall i i' k TX T2, closed i' 0 k T2 ->
-    subst TX (open_rec i (varH 0) T2) = open_rec i TX T2.
-Proof.
-  intros. generalize dependent i'. generalize dependent i.
-  induction T2; intros; inversion H; simpl; eauto;
-  try solve [rewrite (IHT2_1 _ i'); eauto;
-             rewrite (IHT2_2 _ (S i')); eauto;
-             rewrite (IHT2_2 _ (S i')); eauto];
-  try solve [rewrite (IHT2_1 _ i'); eauto;
-             rewrite (IHT2_2 _ i'); eauto].
-  subst.
-  case_eq (beq_nat x 0); intros E. omega. omega.
-  case_eq (beq_nat i x); intros E. eauto. eauto.
-  erewrite IHT2. reflexivity. eassumption.
-Qed.
-
-Lemma Forall2_length: forall A B f (G1:list A) (G2:list B),
-                        Forall2 f G1 G2 -> length G1 = length G2.
-Proof.
-  intros. induction H.
-  eauto.
-  simpl. eauto.
-Qed.
-
-Lemma nosubst_intro: forall i k T, closed i 0 k T -> nosubst T.
-Proof.
-  intros. generalize dependent i.
-  induction T; intros; inversion H; simpl; eauto.
-  omega.
-Qed.
-
-Lemma nosubst_open: forall i V T2, nosubst (TSel V) -> nosubst T2 -> nosubst (open_rec i V T2).
-Proof.
-  intros. generalize dependent i. induction T2; intros;
-  try inversion H0; simpl; eauto; destruct v; eauto.
-  case_eq (beq_nat i i0); intros E. eauto. eauto.
-Qed.
 
 
 
@@ -1927,7 +947,7 @@ Proof.
     split. { rewrite app_length in *. simpl in *. eapply splice_retreat4.
     eassumption. constructor. eapply indexr_max. eassumption. }
     
-    intros. assert (forall kx : nat, val_type venv0 (GH ++ [jj]) 
+    intros. assert (forall kx : nat, val_type venv (GH ++ [jj]) 
       (open_rec k (varH 0) (splice 0 T1)) kx (jj0 kx) vx).
     intros. specialize (H2 kx). apply unvv. apply vv in H2. eapply IHn; try omega; eassumption.
     specialize (H1 _ _ H3).
@@ -1944,7 +964,7 @@ Proof.
     unfold open in *. simpl in *. apply vv. rewrite val_type_unfold in *. destruct v; try solve by inversion. ev.
     split. { rewrite app_length. simpl. eapply splice_retreat5. constructor. omega. eassumption. }
     split. { rewrite app_length. simpl. eapply splice_retreat5. constructor. omega. eassumption. }
-    intros. assert (forall kx : nat, val_type venv0 GH (open_rec k (varF x) T1) kx (jj0 kx) vx).
+    intros. assert (forall kx : nat, val_type venv GH (open_rec k (varF x) T1) kx (jj0 kx) vx).
     intros. specialize (H2 kx). apply unvv. apply vv in H2. eapply IHn; try omega; eassumption.
     specialize (H1 _ _ H3).
     ev. exists x0. exists x1. split. assumption.
@@ -2006,20 +1026,20 @@ Proof.
     intros. specialize (H2 H3). apply unvv. apply vv in H2. eapply IHn; try omega; eassumption.
 
   - inversion Cz. subst. simpl in *. rewrite app_length in *. apply vv. rewrite val_type_unfold.
-    assert (closed 1 (length GH + length [jj]) (length venv0)
+    assert (closed 1 (length GH + length [jj]) (length venv)
           (open_rec (S k) (varH 0) (splice 0 T)) /\
         (exists jj0 : forall x0 : nat, vset x0,
            jj0 m = d m /\
            (forall n0 : nat,
-            val_type venv0 (jj0 :: GH ++ [jj])
+            val_type venv (jj0 :: GH ++ [jj])
               (open (varH (length GH + length [jj]))
                  (open_rec (S k) (varH 0) (splice 0 T))) n0 (jj0 n0) v))).
                  destruct v; assumption. clear V. ev.
-    assert (closed 1 (length GH) (length venv0) (open_rec (S k) (varF x) T) /\
+    assert (closed 1 (length GH) (length venv) (open_rec (S k) (varF x) T) /\
     (exists jj0 : forall x1 : nat, vset x1,
        jj0 m = d m /\
        (forall n0 : nat,
-        val_type venv0 (jj0 :: GH)
+        val_type venv (jj0 :: GH)
           (open (varH (length GH)) (open_rec (S k) (varF x) T)) n0 (jj0 n0) v))) as Goal.
     split. eapply splice_retreat4. simpl in H. eassumption. 
     constructor. eapply indexr_max. eassumption. 
@@ -2034,19 +1054,19 @@ Proof.
     destruct v; apply Goal.
 
   - inversion Cz. subst. simpl in *. apply vv. rewrite val_type_unfold.
-    assert (closed 1 (length GH) (length venv0) (open_rec (S k) (varF x) T) /\
+    assert (closed 1 (length GH) (length venv) (open_rec (S k) (varF x) T) /\
         (exists jj0 : forall x0 : nat, vset x0,
            jj0 m = d m /\
            (forall n0 : nat,
-            val_type venv0 (jj0 :: GH)
+            val_type venv (jj0 :: GH)
               (open (varH (length GH)) (open_rec (S k) (varF x) T)) n0
               (jj0 n0) v))). destruct v; assumption. clear V. ev.
-    assert (closed 1 (length (GH ++ [jj])) (length venv0)
+    assert (closed 1 (length (GH ++ [jj])) (length venv)
       (open_rec (S k) (varH 0) (splice 0 T)) /\
     (exists jj0 : forall x1 : nat, vset x1,
        jj0 m = d m /\
        (forall n0 : nat,
-        val_type venv0 (jj0 :: GH ++ [jj])
+        val_type venv (jj0 :: GH ++ [jj])
           (open (varH (length (GH ++ [jj])))
              (open_rec (S k) (varH 0) (splice 0 T))) n0 (jj0 n0) v))) as Goal.
     split. rewrite app_length. eapply splice_retreat5. constructor. omega. eassumption.
@@ -2062,19 +1082,19 @@ Proof.
     destruct v; apply Goal.
 
   - inversion Cz. subst. rewrite app_length in *. simpl in *. apply vv. rewrite val_type_unfold.
-    assert (val_type venv0 (GH ++ [jj]) (open_rec k (varH 0) (splice 0 T1)) m (d m) v /\
-        val_type venv0 (GH ++ [jj]) (open_rec k (varH 0) (splice 0 T2)) m (d m) v). destruct v; assumption. clear V. ev.
-    assert (val_type venv0 GH (open_rec k (varF x) T1) m (d m) v /\
-    val_type venv0 GH (open_rec k (varF x) T2) m (d m) v) as Goal. 
+    assert (val_type venv (GH ++ [jj]) (open_rec k (varH 0) (splice 0 T1)) m (d m) v /\
+        val_type venv (GH ++ [jj]) (open_rec k (varH 0) (splice 0 T2)) m (d m) v). destruct v; assumption. clear V. ev.
+    assert (val_type venv GH (open_rec k (varF x) T1) m (d m) v /\
+    val_type venv GH (open_rec k (varF x) T2) m (d m) v) as Goal. 
     split. apply unvv. apply vv in H. eapply IHn; try eassumption; try omega.
     apply unvv. apply vv in H0. eapply IHn; try eassumption; try omega.
     destruct v; apply Goal.
 
   - inversion Cz. subst. simpl in *. apply vv. rewrite val_type_unfold.
-    assert (val_type venv0 GH (open_rec k (varF x) T1) m (d m) v /\
-        val_type venv0 GH (open_rec k (varF x) T2) m (d m) v). destruct v; assumption. clear V. ev.
-    assert (val_type venv0 (GH ++ [jj]) (open_rec k (varH 0) (splice 0 T1)) m (d m) v /\
-    val_type venv0 (GH ++ [jj]) (open_rec k (varH 0) (splice 0 T2)) m (d m) v) as Goal.
+    assert (val_type venv GH (open_rec k (varF x) T1) m (d m) v /\
+        val_type venv GH (open_rec k (varF x) T2) m (d m) v). destruct v; assumption. clear V. ev.
+    assert (val_type venv (GH ++ [jj]) (open_rec k (varH 0) (splice 0 T1)) m (d m) v /\
+    val_type venv (GH ++ [jj]) (open_rec k (varH 0) (splice 0 T2)) m (d m) v) as Goal.
     split. apply unvv. apply vv in H. eapply IHn; try eassumption; try omega.
     apply unvv. apply vv in H0. eapply IHn; try eassumption; try omega.
     destruct v; apply Goal.
@@ -2135,9 +1155,9 @@ Lemma vtp_subst3: forall venv jj v T2 d k,
   val_type venv [jj] (open (varH 0) T2) k (d k) v.
 Proof.
   intros. apply unvv. assert (splice 0 T2 = T2) as EE. eapply closed_splice_idem. eassumption. omega.
-  assert (vtp (jj::venv0) ([] ++ [jj]) (open (varH 0) (splice 0 T2)) k (d k) v).
-  assert (indexr (length venv0) (jj :: venv0) = Some jj). simpl. 
-    replace (beq_nat (length venv0) (length venv0) ) with true. reflexivity. 
+  assert (vtp (jj::venv) ([] ++ [jj]) (open (varH 0) (splice 0 T2)) k (d k) v).
+  assert (indexr (length venv) (jj :: venv) = Some jj). simpl. 
+    replace (beq_nat (length venv) (length venv) ) with true. reflexivity. 
     apply beq_nat_refl. 
   eapply vtp_subst. simpl. eapply closed_upgrade_freef. eassumption. omega. eassumption.
   apply vv. assumption. 
@@ -2454,7 +1474,7 @@ Proof.
   induction W; intros ? ? WFE; inversion Heqe; try subst x0.
 
   - Case "Var". 
-    destruct (indexr_safe_ex venv0 renv env T1 x) as [d [v [I [D V]]]]. eauto. eauto. 
+    destruct (indexr_safe_ex venv renv env T1 x) as [d [v [I [D V]]]]. eauto. eauto. 
     
     exists d. exists v. split. exists 0. intros. destruct n. omega. simpl. rewrite I. eauto. split. apply I. split. apply D. eapply V.
 
@@ -2468,8 +1488,8 @@ Proof.
     destruct v; split; try assumption; exists d; (split; [reflexivity| assumption]). 
 
   - Case "And".
-    destruct (IHW1 eq_refl venv0 renv WFE) as [d1 [v1 [E1 [I1 [D1 HVF]]]]].
-    destruct (IHW2 eq_refl venv0 renv WFE) as [d2 [v2 [E2 [I2 [D2 HVX]]]]].
+    destruct (IHW1 eq_refl venv renv WFE) as [d1 [v1 [E1 [I1 [D1 HVF]]]]].
+    destruct (IHW2 eq_refl venv renv WFE) as [d2 [v2 [E2 [I2 [D2 HVX]]]]].
     rewrite I1 in I2. inversion I2. subst v2.
     rewrite D1 in D2. inversion D2. subst d2.
     exists d1. exists v1.
@@ -2477,7 +1497,7 @@ Proof.
     intros. rewrite val_type_unfold. destruct v1; (split; [apply HVF|apply HVX]).
 
   - Case "Sub".
-    specialize (IHW Heqe venv0 renv WFE). ev. exists x0. exists x1. split. subst e. eassumption. split. assumption. split. assumption. 
+    specialize (IHW Heqe venv renv WFE). ev. exists x0. exists x1. split. subst e. eassumption. split. assumption. split. assumption. 
     intros. eapply unvv. eapply valtp_widen. eapply H4. eapply H. eapply WFE. 
 Qed. 
 
@@ -2491,16 +1511,16 @@ Proof.
   induction W; intros ? ? WFE.
 
   - Case "Var".
-    destruct (invert_var x env T1 (t_var x env T1 H H0) venv0 renv WFE) as [d [v [E [I [D V]]]]].
+    destruct (invert_var x env T1 (t_var x env T1 H H0) venv renv WFE) as [d [v [E [I [D V]]]]].
     exists d. exists v. split. apply E. apply V.
   - Case "VarPack". 
-    destruct (invert_var x G1 (TBind T1) (t_var_pack _ x T1 T1' H H0 H1) venv0 renv WFE) as [d [v [E [I [D V]]]]].
+    destruct (invert_var x G1 (TBind T1) (t_var_pack _ x T1 T1' H H0 H1) venv renv WFE) as [d [v [E [I [D V]]]]].
     exists d. exists v. split. apply E. apply V. 
 
 
   - Case "unpack". 
     rewrite <-(wf_length2 _ _ _ WFE) in H. 
-    destruct (IHW1 venv0 renv WFE) as [dx [vx [IW1 HVX]]].
+    destruct (IHW1 venv renv WFE) as [dx [vx [IW1 HVX]]].
     specialize (HVX 0).
     rewrite val_type_unfold in HVX.
     assert (exists jj : vseta,
@@ -2513,7 +1533,7 @@ Proof.
       intros. eapply vtp_subst2. assumption. eapply unvv. eapply valtp_extend. eapply VXH.
       eapply indexr_hit2. reflexivity. reflexivity. } 
     
-    assert (R_env (vx::venv0) (jj::renv) (T1'::env)) as WFE1.
+    assert (R_env (vx::venv) (jj::renv) (T1'::env)) as WFE1.
     eapply wf_env_extend. assumption. rewrite H. assumption.
 
     specialize (IHW2 _ _ WFE1).
@@ -2531,7 +1551,7 @@ Proof.
     eapply HVY. rewrite (wf_length2 _ _ _ WFE). assumption.
 
   - Case "And". 
-    destruct (invert_var x env (TAnd T1 T2) (t_and env x T1 T2 W1 W2) venv0 renv WFE) as [d [v [E [I [D V]]]]].
+    destruct (invert_var x env (TAnd T1 T2) (t_and env x T1 T2 W1 W2) venv renv WFE) as [d [v [E [I [D V]]]]].
     exists d. exists v. split. apply E. apply V. 
 
   - Case "Typ".
@@ -2539,7 +1559,7 @@ Proof.
     specialize valtp_to_vseta. intros S. specialize (S renv [] T1). ev. 
     
     exists x. eexists. split. exists 1. intros. destruct n. inversion H1. simpl. reflexivity.
-    rewrite <-(wf_length2 venv0 renv) in H.
+    rewrite <-(wf_length2 venv renv) in H.
     intros. rewrite val_type_unfold. simpl. repeat split; try eapply H.
     destruct k. trivial. intros. destruct (H0 k (dy k) vy). split; assumption. 
     eapply WFE.
@@ -2547,8 +1567,8 @@ Proof.
     
   - Case "App".
     rewrite <-(wf_length2 _ _ _ WFE) in H. 
-    destruct (IHW1 venv0 renv WFE) as [df [vf [IW1 HVF]]].
-    destruct (IHW2 venv0 renv WFE) as [dx [vx [IW2 HVX]]].
+    destruct (IHW1 venv renv WFE) as [df [vf [IW1 HVF]]].
+    destruct (IHW2 venv renv WFE) as [dx [vx [IW2 HVX]]].
 
     specialize (HVF 0).
     rewrite val_type_unfold in HVF.
@@ -2570,8 +1590,8 @@ Proof.
 
   - Case "DApp".
     rewrite <-(wf_length2 _ _ _ WFE) in H0. 
-    destruct (IHW1 venv0 renv WFE) as [df [vf [IW1 HVF]]].
-    destruct (invert_var x env T1 W2 venv0 renv WFE) as [dx [vx [IW2 [I [D HVX]]]]].
+    destruct (IHW1 venv renv WFE) as [df [vf [IW1 HVF]]].
+    destruct (invert_var x env T1 W2 venv renv WFE) as [dx [vx [IW2 [I [D HVX]]]]].
 
     specialize (HVF 0).
     rewrite val_type_unfold in HVF.
@@ -2602,15 +1622,15 @@ Proof.
     eexists. split. exists 0. intros. destruct n. omega. simpl. eauto.
     intros. rewrite val_type_unfold. repeat split; eauto.
     intros.
-    assert (R_env (vx::venv0) (jj::renv) (T1::env)) as WFE1. {
+    assert (R_env (vx::venv) (jj::renv) (T1::env)) as WFE1. {
       eapply wf_env_extend0. eapply WFE. eapply H0. }
-    specialize (IHW (vx::venv0) (jj::renv) WFE1).
+    specialize (IHW (vx::venv) (jj::renv) WFE1).
     destruct IHW as [d [v [EV VT]]]. rewrite <-(wf_length2 _ _ _ WFE) in VT. 
     exists d. exists v. split. eapply EV. 
     intros. eapply vtp_subst3. assumption. eapply VT. 
 
   - Case "Sub".
-    specialize (IHW venv0 renv WFE). ev. exists x. exists x0. split. eassumption.
+    specialize (IHW venv renv WFE). ev. exists x. exists x0. split. eassumption.
     intros. eapply unvv. eapply valtp_widen. eapply H1. eapply H. eapply WFE. 
 
 Grab Existential Variables.
