ecoop17/dsubsup_total_rec_base.v
@@ -1,0 +1,372 @@
+(* Only syntax basics, no logical relations. *)
+(*
+ DSub (D<:) + Bot + /\ + { z => ... }
+ T ::= Top | Bot | x.Type | { Type: S..U } | (z: T) -> T^z | T1 /\ T2 | { z => T^z }
+ t ::= x | { Type = T } | lambda x:T.t | t t | unpack(t) { x => t }
+ *)
+
+Require Export SfLib.
+
+Require Export Arith.EqNat.
+Require Export Arith.Le.
+Require Export Omega.
+
+(* ### Syntax ### *)
+
+Definition id := nat.
+
+(* term variables occurring in types *)
+Inductive var : Type :=
+| varF : id -> var (* free, in concrete environment *)
+| varH : id -> var (* free, in abstract environment  *)
+| varB : id -> var (* locally-bound variable *)
+.
+
+Inductive ty : Type :=
+| TTop : ty
+| TBot : ty
+(* (z: T) -> T^z *)
+| TAll : ty -> ty -> ty
+(* x.Type *)
+| TSel : var -> ty
+(* { Type: S..U } *)
+| TMem : ty(*S*) -> ty(*U*) -> ty
+| TBind  : ty -> ty (* Recursive binder: { z => T^z },
+                         where z is locally bound in T *)
+| TAnd : ty -> ty -> ty (* Intersection Type: T1 /\ T2 *)
+.
+
+Inductive tm : Type :=
+(* x -- free variable, matching concrete environment *)
+| tvar : id -> tm
+(* { Type = T } *)
+| ttyp : ty -> tm
+(* lambda x:T.t *)
+| tabs : ty -> tm -> tm
+(* t t *)
+| tapp : tm -> tm -> tm
+(* unpack(e) { x => ... } *)
+| tunpack : tm -> tm -> tm                       
+.
+
+Inductive vl : Type :=
+(* a closure for a lambda abstraction *)
+| vabs : list vl (*H*) -> ty -> tm -> vl
+(* a closure for a first-class type *)
+| vty : list vl (*H*) -> ty -> vl
+.
+
+Definition tenv := list ty. (* Gamma environment: static *)
+Definition venv := list vl. (* H environment: run-time *)
+
+
+(* ### Representation of Bindings ### *)
+
+(* An environment is a list of values, indexed by decrementing ids. *)
+
+Fixpoint indexr {X : Type} (n : id) (l : list X) : option X :=
+  match l with
+    | [] => None
+    | a :: l' =>
+      if (beq_nat n (length l')) then Some a else indexr n l'
+  end.
+
+Inductive closed: nat(*B*) -> nat(*H*) -> nat(*F*) -> ty -> Prop :=
+| cl_top: forall i j k,
+    closed i j k TTop
+| cl_bot: forall i j k,
+    closed i j k TBot
+| cl_all: forall i j k T1 T2,
+    closed i j k T1 ->
+    closed (S i) j k T2 ->
+    closed i j k (TAll T1 T2)
+| cl_sel: forall i j k x,
+    k > x ->
+    closed i j k (TSel (varF x))
+| cl_selh: forall i j k x,
+    j > x ->
+    closed i j k (TSel (varH x))
+| cl_selb: forall i j k x,
+    i > x ->
+    closed i j k (TSel (varB x))
+| cl_mem: forall i j k T1 T2,
+    closed i j k T1 ->
+    closed i j k T2 ->
+    closed i j k (TMem T1 T2)
+| cl_bind: forall i j k T,
+    closed (S i) j k T ->
+    closed i j k (TBind T)
+| cl_and: forall i j k T1 T2,
+    closed i j k T1 ->
+    closed i j k T2 ->
+    closed i j k (TAnd T1 T2)
+.
+
+(* open define a locally-nameless encoding wrt to TVarB type variables. *)
+(* substitute var u for all occurrences of (varB k) *)
+Fixpoint open_rec (k: nat) (u: var) (T: ty) { struct T }: ty :=
+  match T with
+    | TTop        => TTop
+    | TBot        => TBot
+    | TAll T1 T2  => TAll (open_rec k u T1) (open_rec (S k) u T2)
+    | TSel (varF x) => TSel (varF x)
+    | TSel (varH i) => TSel (varH i)
+    | TSel (varB i) => if beq_nat k i then TSel u else TSel (varB i)
+    | TMem T1 T2  => TMem (open_rec k u T1) (open_rec k u T2)
+    | TBind T => TBind (open_rec (S k) u T)
+    | TAnd T1 T2 => TAnd (open_rec k u T1) (open_rec k u T2)
+  end.
+
+Definition open u T := open_rec 0 u T.
+
+(* Locally-nameless encoding with respect to varH variables. *)
+Fixpoint subst (U : var) (T : ty) {struct T} : ty :=
+  match T with
+    | TTop         => TTop
+    | TBot         => TBot
+    | TAll T1 T2   => TAll (subst U T1) (subst U T2)
+    | TSel (varB i) => TSel (varB i)
+    | TSel (varF i) => TSel (varF i)
+    | TSel (varH i) => if beq_nat i 0 then TSel U else TSel (varH (i-1))
+    | TMem T1 T2     => TMem (subst U T1) (subst U T2)
+    | TBind T       => TBind (subst U T)
+    | TAnd T1 T2    => TAnd (subst U T1)(subst U T2)
+  end.
+
+Fixpoint nosubst (T : ty) {struct T} : Prop :=
+  match T with
+    | TTop         => True
+    | TBot         => True
+    | TAll T1 T2   => nosubst T1 /\ nosubst T2
+    | TSel (varB i) => True
+    | TSel (varF i) => True
+    | TSel (varH i) => i <> 0
+    | TMem T1 T2    => nosubst T1 /\ nosubst T2
+    | TBind T       => nosubst T
+    | TAnd T1 T2    => nosubst T1 /\ nosubst T2
+  end.
+
+(* ### Subtyping ### *)
+(*
+Note: In contrast to the rules on paper, the subtyping 
+relation has two environments instead of just one.
+(The same holds for the semantic types, val_type, below).
+This split into an abstract and a concrete environment
+was necessary in the D<: soundness development, but is 
+not required here. We just keep it for consistency with
+our earlier Coq files.
+
+The first env is for looking up varF variables.
+The first env matches the concrete runtime environment, and is
+extended during type assignment.
+The second env is for looking up varH variables.
+The second env matches the abstract runtime environment, and is
+extended during subtyping.
+*)
+Inductive stp: tenv -> tenv -> ty -> ty -> Prop :=
+| stp_top: forall G1 GH T1,
+    closed 0 (length GH) (length G1) T1 ->
+    stp G1 GH T1 TTop
+| stp_bot: forall G1 GH T2,
+    closed 0 (length GH) (length G1) T2 ->
+    stp G1 GH TBot T2
+| stp_mem: forall G1 GH S1 U1 S2 U2,
+    stp G1 GH U1 U2 ->
+    stp G1 GH S2 S1 ->
+    stp G1 GH (TMem S1 U1) (TMem S2 U2)
+| stp_sel1: forall G1 GH TX T2 x,
+    indexr x G1 = Some TX ->
+    closed 0 0 (length G1) TX ->
+    stp G1 GH TX (TMem TBot T2) ->
+    stp G1 GH (TSel (varF x)) T2
+| stp_sel2: forall G1 GH TX T1 x,
+    indexr x G1 = Some TX ->
+    closed 0 0 (length G1) TX ->
+    stp G1 GH TX (TMem T1 TTop) ->
+    stp G1 GH T1 (TSel (varF x)) 
+| stp_selx: forall G1 GH v x,
+    indexr x G1 = Some v ->
+    stp G1 GH (TSel (varF x)) (TSel (varF x))
+| stp_sela1: forall G1 GH TX T2 x,
+    indexr x GH = Some TX ->
+    closed 0 x (length G1) TX ->
+    stp G1 GH TX (TMem TBot T2) ->
+    stp G1 GH (TSel (varH x)) T2
+| stp_sela2: forall G1 GH TX T1 x,
+    indexr x GH = Some TX ->
+    closed 0 x (length G1) TX ->
+    stp G1 GH TX (TMem T1 TTop) ->
+    stp G1 GH T1 (TSel (varH x)) 
+| stp_selax: forall G1 GH v x,
+    indexr x GH = Some v  ->
+    stp G1 GH (TSel (varH x)) (TSel (varH x))
+
+(* stp for recursive types and intersection types *)
+| stp_bindx: forall GH G1 T1 T1' T2 T2',
+    stp G1 (T1'::GH) T1' T2' ->
+    T1' = (open (varH (length GH)) T1) ->
+    T2' = (open (varH (length GH)) T2) ->
+    closed 1 (length GH) (length G1) T1 ->
+    closed 1 (length GH) (length G1) T2 ->
+    stp G1 GH (TBind T1) (TBind T2)
+
+| stp_and11: forall GH G1 T1 T2 T,
+    stp G1 GH T1 T ->
+    closed 0 (length GH) (length G1) T2 ->
+    stp G1 GH (TAnd T1 T2) T
+
+| stp_and12: forall GH G1 T1 T2 T,
+    stp G1 GH T2 T ->
+    closed 0 (length GH) (length G1) T1 ->
+    stp G1 GH (TAnd T1 T2) T
+
+| stp_and2: forall GH G1 T1 T2 T,
+    stp G1 GH T T1 ->
+    stp G1 GH T T2 ->
+    stp G1 GH T (TAnd T1 T2)
+
+
+| stp_all: forall G1 GH T1 T2 T3 T4 x,
+    stp G1 GH T3 T1 ->
+    x = length GH ->
+    closed 1 (length GH) (length G1) T2 ->
+    closed 1 (length GH) (length G1) T4 ->
+    stp G1 (T3::GH) (open (varH x) T2) (open (varH x) T4) ->
+    stp G1 GH (TAll T1 T2) (TAll T3 T4)
+| stp_trans: forall G1 GH T1 T2 T3,
+    stp G1 GH T1 T2 ->
+    stp G1 GH T2 T3 ->
+    stp G1 GH T1 T3
+.
+
+(* ### Type Assignment ### *)
+Inductive has_type : tenv -> tm -> ty -> Prop :=
+| t_var: forall x env T1,
+           indexr x env = Some T1 ->
+           stp env [] T1 T1 ->
+           has_type env (tvar x) T1
+(* pack a recursive type  *)
+| t_var_pack : forall G1 x T1 T1',
+           (* has_type G1 (tvar x) T1' -> *)
+           indexr x G1 = Some (open (varF x) T1) ->            
+           T1' = (open (varF x) T1) ->
+           closed 1 0 (length G1) T1 ->
+           has_type G1 (tvar x) (TBind T1) 
+(* unpack a recursive type: unpack(x:{z=>T^z}) { x:T^x => ... }  *)                    
+| t_unpack: forall env x y T1 T1' T2,
+           has_type env x (TBind T1) ->
+           T1' = (open (varF (length env)) T1) ->
+           has_type (T1'::env) y T2 ->
+           closed 0 0 (length env) T2 ->
+           has_type env (tunpack x y) T2
+
+(* intersection typing *)
+| t_and : forall env x T1 T2,
+           has_type env (tvar x) T1 ->
+           has_type env (tvar x) T2 ->
+           has_type env (tvar x) (TAnd T1 T2)
+
+               
+| t_typ: forall env T1,
+           closed 0 0 (length env) T1 ->
+           has_type env (ttyp T1) (TMem T1 T1)
+               
+| t_app: forall env f x T1 T2,
+           has_type env f (TAll T1 T2) ->
+           has_type env x T1 ->
+           closed 0 0 (length env) T2 ->
+           has_type env (tapp f x) T2
+| t_dapp:forall env f x T1 T2 T,
+           has_type env f (TAll T1 T2) ->
+           has_type env (tvar x) T1 ->
+           T = open (varF x) T2 ->
+           closed 0 0 (length env) T ->
+           has_type env (tapp f (tvar x)) T
+| t_abs: forall env y T1 T2,
+           has_type (T1::env) y (open (varF (length env)) T2) ->
+           closed 0 0 (length env) (TAll T1 T2) ->
+           has_type env (tabs T1 y) (TAll T1 T2)
+| t_sub: forall env e T1 T2,
+           has_type env e T1 ->
+           stp env [] T1 T2 ->
+           has_type env e T2
+.
+
+
+
+(* ### Evaluation (Big-Step Semantics) ### *)
+
+(*
+None             means timeout
+Some None        means stuck
+Some (Some v))   means result v
+Could use do-notation to clean up syntax.
+*)
+
+Fixpoint teval(n: nat)(env: venv)(t: tm){struct n}: option (option vl) :=
+  match n with
+    | 0 => None
+    | S n =>
+      match t with
+        | tvar x       => Some (indexr x env)
+        | ttyp T       => Some (Some (vty env T))
+        | tabs T y     => Some (Some (vabs env T y))
+        | tapp ef ex   =>
+          match teval n env ex with
+            | None => None
+            | Some None => Some None
+            | Some (Some vx) =>
+              match teval n env ef with
+                | None => None
+                | Some None => Some None
+                | Some (Some (vty _ _)) => Some None
+                | Some (Some (vabs env2 _ ey)) =>
+                  teval n (vx::env2) ey
+              end
+          end
+        | tunpack ex ey =>
+          match teval n env ex with
+            | None => None
+            | Some None => Some None
+            | Some (Some vx) =>
+              teval n (vx::env) ey 
+          end
+      end
+  end.
+
+
+Definition tevaln env e v := exists nm, forall n, n > nm -> teval n env e = Some (Some v).
+
+
+Fixpoint tsize_flat(T: ty) :=
+  match T with
+    | TTop => 1
+    | TBot => 1
+    | TAll T1 T2 => S (tsize_flat T1 + tsize_flat T2)
+    | TSel _ => 1
+    | TMem T1 T2 => S (tsize_flat T1 + tsize_flat T2)	
+    | TBind T => S (tsize_flat T)
+    | TAnd T1 T2 => S (tsize_flat T1 + tsize_flat T2)
+  end. 
+
+Lemma open_preserves_size: forall T x j,
+  tsize_flat T = tsize_flat (open_rec j (varH x) T).
+Proof.
+  intros T. induction T; intros; simpl; eauto.
+  - destruct v; simpl; destruct (beq_nat j i); eauto.
+Qed.
+
+
+
+
+Ltac ev := repeat match goal with
+                    | H: exists _, _ |- _ => destruct H
+                    | H: _ /\  _ |- _ => destruct H
+           end.
+
+Ltac inv_mem := match goal with
+                  | H: closed 0 (length ?GH) (length ?G) (TMem ?T1 ?T2) |-
+                    closed 0 (length ?GH) (length ?G) ?T2 => inversion H; subst; eauto
+                  | H: closed 0 (length ?GH) (length ?G) (TMem ?T1 ?T2) |-
+                    closed 0 (length ?GH) (length ?G) ?T1 => inversion H; subst; eauto
+                end.
