ecoop17/dsubsup_total_rec_binding.v
@@ -1,0 +1,870 @@
+Require Import dsubsup_total_rec_base.
+Require Import FunctionalExtensionality.
+Ltac inverse H := (inversion H; subst).
+Ltac match_case_analysis :=
+  repeat
+    match goal with
+    | H : context f [match ?x with _ => _ end] |- _ =>
+      destruct x; try solve [inverse H]
+    end.
+
+Ltac match_case_analysis_goal :=
+  repeat
+    match goal with
+    | |- context f [match ?x with _ => _ end] =>
+      destruct x
+    end.
+
+Ltac match_case_analysis_eauto :=
+  repeat
+    match goal with
+    | H : context f [match ?x with _ => _ end] |- _ =>
+      destruct x; try solve [inverse H; eauto]
+    end.
+
+
+(* Safer version of split; for use in automation. *)
+Ltac split_conj :=
+  repeat match goal with
+  | |- _ /\ _ => split
+  end.
+
+Hint Unfold open.
+Hint Unfold indexr.
+Hint Unfold length.
+
+
+Hint Constructors ty.
+Hint Constructors tm.
+Hint Constructors vl.
+
+Hint Constructors closed.
+Hint Constructors has_type.
+Hint Constructors stp.
+
+Hint Constructors option.
+Hint Constructors list.
+
+Hint Resolve ex_intro.
+
+(* ############################################################ *)
+(* Examples *)
+(* ############################################################ *)
+
+
+Ltac crush :=
+  try solve [eapply stp_selx; compute; eauto; crush];
+  try solve [eapply stp_selax; compute; eauto; crush];
+  try solve [econstructor; compute; eauto; crush];
+  try solve [eapply t_sub; crush].
+
+(* define polymorphic identity function *)
+
+Definition polyId := TAll (TMem TBot TTop) (TAll (TSel (varB 0)) (TSel (varB 1))).
+
+Example ex10: has_type [] (tabs (TMem TBot TTop) (tabs (TSel (varF 0)) (tvar 1))) polyId.
+Proof.
+  crush.
+Qed.
+
+
+(* instantiate it to TTop *)
+(* Example ex20: has_type [polyId] (tapp (tvar 0) (ttyp TTop)) (TAll TTop TTop). *)
+(* Proof. *)
+(*   crush. *)
+(* Qed. *)
+
+
+Lemma indexr_max : forall X vs n (T: X),
+                       indexr n vs = Some T ->
+                       n < length vs.
+Proof.
+  intros X vs. induction vs.
+  - Case "nil". intros. inversion H.
+  - Case "cons".
+    intros. inversion H.
+    case_eq (beq_nat n (length vs)); intros E2.
+    + SSCase "hit".
+      eapply beq_nat_true in E2. subst n. compute. eauto.
+    + SSCase "miss".
+      rewrite E2 in H1.
+      assert (n < length vs). eapply IHvs. apply H1.
+      compute. eauto.
+Qed.
+
+Lemma le_xx : forall a b,
+                       a <= b ->
+                       exists E, le_lt_dec a b = left E.
+Proof. intros.
+  case_eq (le_lt_dec a b). intros. eauto.
+  intros. omega.
+Qed.
+Lemma le_yy : forall a b,
+                       a > b ->
+                       exists E, le_lt_dec a b = right E.
+Proof. intros.
+  case_eq (le_lt_dec a b). intros. omega.
+  intros. eauto.
+Qed.
+
+Lemma indexr_extend : forall X vs n x (T: X),
+                       indexr n vs = Some T ->
+                       indexr n (x::vs) = Some T.
+
+Proof.
+  intros.
+  assert (n < length vs). eapply indexr_max. eauto.
+  assert (beq_nat n (length vs) = false) as E. eapply beq_nat_false_iff. omega.
+  unfold indexr. unfold indexr in H. rewrite H. rewrite E. reflexivity.
+Qed.
+
+(* splicing -- for stp_extend. *)
+
+Fixpoint splice n (T : ty) {struct T} : ty :=
+  match T with
+    | TTop         => TTop
+    | TBot         => TBot
+    | TAll T1 T2   => TAll (splice n T1) (splice n T2)
+    | TSel (varF i) => TSel (varF i)
+    | TSel (varB i) => TSel (varB i)
+    | TSel (varH i) => if le_lt_dec n i then TSel (varH (i+1)) else TSel (varH i)
+    | TMem T1 T2   => TMem (splice n T1) (splice n T2)
+    | TBind T      => TBind (splice n T)
+    | TAnd T1 T2   => TAnd (splice n T1) (splice n T2)
+  end.
+
+Definition spliceat n (V: (venv*ty)) :=
+  match V with
+    | (G,T) => (G,splice n T)
+  end.
+
+Lemma splice_open_permute: forall {X} (G0:list X) T2 n j,
+(open_rec j (varH (n + S (length G0))) (splice (length G0) T2)) =
+(splice (length G0) (open_rec j (varH (n + length G0)) T2)).
+Proof.
+  intros X G T. induction T; intros; simpl; eauto;
+  try rewrite IHT1; try rewrite IHT2; try rewrite IHT; eauto;
+  destruct v; eauto.
+
+  case_eq (le_lt_dec (length G) i); intros E LE; simpl; eauto.
+  rewrite LE. eauto.
+  rewrite LE. eauto.
+  case_eq (beq_nat j i); intros E; simpl; eauto.
+  case_eq (le_lt_dec (length G) (n + length G)); intros EL LE.
+  rewrite E.
+  assert (n + S (length G) = n + length G + 1). omega.
+  rewrite H. eauto.
+  omega.
+  rewrite E. eauto.
+Qed.
+
+Lemma indexr_splice_hi: forall G0 G2 x0 v1 T,
+    indexr x0 (G2 ++ G0) = Some T ->
+    length G0 <= x0 ->
+    indexr (x0 + 1) (map (splice (length G0)) G2 ++ v1 :: G0) = Some (splice (length G0) T).
+Proof.
+  intros G0 G2. induction G2; intros.
+  - eapply indexr_max in H. simpl in H. omega.
+  - simpl in H.
+    case_eq (beq_nat x0 (length (G2 ++ G0))); intros E.
+    + rewrite E in H. inversion H. subst. simpl.
+      rewrite app_length in E.
+      rewrite app_length. rewrite map_length. simpl.
+      assert (beq_nat (x0 + 1) (length G2 + S (length G0)) = true). {
+        eapply beq_nat_true_iff. eapply beq_nat_true_iff in E. omega.
+      }
+      rewrite H1. eauto.
+    + rewrite E in H.  eapply IHG2 in H. eapply indexr_extend. eapply H. eauto.
+Qed.
+
+Lemma indexr_spliceat_hi: forall G0 G2 x0 v1 G T,
+    indexr x0 (G2 ++ G0) = Some (G, T) ->
+    length G0 <= x0 ->
+    indexr (x0 + 1) (map (spliceat (length G0)) G2 ++ v1 :: G0) =
+    Some (G, splice (length G0) T).
+Proof.
+  intros G0 G2. induction G2; intros.
+  - eapply indexr_max in H. simpl in H. omega.
+  - simpl in H. destruct a.
+    case_eq (beq_nat x0 (length (G2 ++ G0))); intros E.
+    + rewrite E in H. inversion H. subst. simpl.
+      rewrite app_length in E.
+      rewrite app_length. rewrite map_length. simpl.
+      assert (beq_nat (x0 + 1) (length G2 + S (length G0)) = true). {
+        eapply beq_nat_true_iff. eapply beq_nat_true_iff in E. omega.
+      }
+      rewrite H1. eauto.
+    + rewrite E in H.  eapply IHG2 in H. eapply indexr_extend. eapply H. eauto.
+Qed.
+
+Lemma plus_lt_contra: forall a b,
+  a + b < b -> False.
+Proof.
+  intros a b H. induction a.
+  - simpl in H. apply lt_irrefl in H. assumption.
+  - simpl in H. apply IHa. omega.
+Qed.
+
+Lemma indexr_splice_lo0: forall {X} G0 G2 x0 (T:X),
+    indexr x0 (G2 ++ G0) = Some T ->
+    x0 < length G0 ->
+    indexr x0 G0 = Some T.
+Proof.
+  intros X G0 G2. induction G2; intros.
+  - simpl in H. apply H.
+  - simpl in H.
+    case_eq (beq_nat x0 (length (G2 ++ G0))); intros E.
+    + eapply beq_nat_true_iff in E. subst.
+      rewrite app_length in H0. apply plus_lt_contra in H0. inversion H0.
+    + rewrite E in H. apply IHG2. apply H. apply H0.
+Qed.
+
+Lemma indexr_extend_mult: forall {X} G0 G2 x0 (T:X),
+    indexr x0 G0 = Some T ->
+    indexr x0 (G2++G0) = Some T.
+Proof.
+  intros X G0 G2. induction G2; intros.
+  - simpl. assumption.
+  - simpl.
+    case_eq (beq_nat x0 (length (G2 ++ G0))); intros E.
+    + eapply beq_nat_true_iff in E.
+      apply indexr_max in H. subst.
+      rewrite app_length in H. apply plus_lt_contra in H. inversion H.
+    + apply IHG2. assumption.
+Qed.
+
+Lemma indexr_splice_lo: forall G0 G2 x0 v1 T f,
+    indexr x0 (G2 ++ G0) = Some T ->
+    x0 < length G0 ->
+    indexr x0 (map (splice f) G2 ++ v1 :: G0) = Some T.
+Proof.
+  intros.
+  assert (indexr x0 G0 = Some T). eapply indexr_splice_lo0; eauto.
+  eapply indexr_extend_mult. eapply indexr_extend. eauto.
+Qed.
+
+Lemma indexr_spliceat_lo: forall G0 G2 x0 v1 G T f,
+    indexr x0 (G2 ++ G0) = Some (G, T) ->
+    x0 < length G0 ->
+    indexr x0 (map (spliceat f) G2 ++ v1 :: G0) = Some (G, T).
+Proof.
+  intros.
+  assert (indexr x0 G0 = Some (G, T)). eapply indexr_splice_lo0; eauto.
+  eapply indexr_extend_mult. eapply indexr_extend. eauto.
+Qed.
+
+Lemma closed_splice: forall i j k T n,
+  closed i j k T ->
+  closed i (S j) k (splice n T).
+Proof.
+  intros. induction H; simpl; eauto.
+  case_eq (le_lt_dec n x); intros E LE.
+  apply cl_selh. omega.
+  apply cl_selh. omega.
+Qed.
+
+Lemma map_splice_length_inc: forall G0 G2 v1,
+   (length (map (splice (length G0)) G2 ++ v1 :: G0)) = (S (length (G2 ++ G0))).
+Proof.
+  intros. rewrite app_length. rewrite map_length. induction G2.
+  - simpl. reflexivity.
+  - simpl. eauto.
+Qed.
+
+Lemma map_spliceat_length_inc: forall G0 G2 v1,
+   (length (map (spliceat (length G0)) G2 ++ v1 :: G0)) = (S (length (G2 ++ G0))).
+Proof.
+  intros. rewrite app_length. rewrite map_length. induction G2.
+  - simpl. reflexivity.
+  - simpl. eauto.
+Qed.
+
+Lemma closed_inc_mult: forall i j k T,
+  closed i j k T ->
+  forall i' j' k',
+  i' >= i -> j' >= j -> k' >= k ->
+  closed i' j' k' T.
+Proof.
+  intros i j k T H. induction H; intros; eauto; try solve [constructor; omega].
+  - apply cl_all. apply IHclosed1; omega. apply IHclosed2; omega.
+  - constructor. apply IHclosed; omega.
+Qed.
+
+Lemma closed_inc: forall i j k T,
+  closed i j k T ->
+  closed i (S j) k T.
+Proof.
+  intros. apply (closed_inc_mult i j k T H i (S j) k); omega.
+Qed.
+
+Lemma closed_splice_idem: forall i j k T n,
+                            closed i j k T ->
+                            n >= j ->
+                            splice n T = T.
+Proof.
+  intros. induction H; eauto.
+  - (* TAll *) simpl.
+    rewrite IHclosed1. rewrite IHclosed2.
+    reflexivity.
+    assumption. assumption.
+  - (* TVarH *) simpl.
+    case_eq (le_lt_dec n x); intros E LE. omega. reflexivity.
+  - (* TMem *) simpl.
+    rewrite IHclosed1. rewrite IHclosed2.
+    reflexivity.
+    assumption. assumption.
+  - simpl. rewrite IHclosed. reflexivity. assumption.
+  - simpl. rewrite IHclosed1. rewrite IHclosed2. reflexivity. assumption. assumption.
+Qed.
+
+Lemma stp_closed : forall G GH T1 T2,
+                     stp G GH T1 T2 ->
+                     closed 0 (length GH) (length G) T1 /\ closed 0 (length GH) (length G) T2.
+Proof.
+  intros. induction H;
+    try solve [repeat ev; split; try inv_mem; eauto using indexr_max].
+Qed.
+
+Lemma stp_closed2 : forall G1 GH T1 T2,
+                       stp G1 GH T1 T2 ->
+                       closed 0 (length GH) (length G1) T2.
+Proof.
+  intros. apply (proj2 (stp_closed G1 GH T1 T2 H)).
+Qed.
+
+Lemma stp_closed1 : forall G1 GH T1 T2,
+                       stp G1 GH T1 T2 ->
+                       closed 0 (length GH) (length G1) T1.
+Proof.
+  intros. apply (proj1 (stp_closed G1 GH T1 T2 H)).
+Qed.
+
+
+Lemma closed_upgrade: forall i j k i' T,
+ closed i j k T ->
+ i' >= i ->
+ closed i' j k T.
+Proof.
+ intros. apply (closed_inc_mult i j k T H i' j k); omega.
+Qed.
+
+Lemma closed_upgrade_free: forall i j k j' T,
+ closed i j k T ->
+ j' >= j ->
+ closed i j' k T.
+Proof.
+ intros. apply (closed_inc_mult i j k T H i j' k); omega.
+Qed.
+
+Lemma closed_upgrade_freef: forall i j k k' T,
+ closed i j k T ->
+ k' >= k ->
+ closed i j k' T.
+Proof.
+ intros. apply (closed_inc_mult i j k T H i j k'); omega.
+Qed.
+
+Lemma closed_open: forall i j k V T, closed (i+1) j k T -> closed i j k (TSel V) ->
+  closed i j k (open_rec i V T).
+Proof.
+  intros. generalize dependent i.
+  induction T; intros; inversion H;
+  try econstructor;
+  try eapply IHT1; eauto; try eapply IHT2; eauto; try eapply IHT; eauto.
+  eapply closed_upgrade. eauto. eauto.
+  - Case "TVarB". simpl.
+    case_eq (beq_nat i x); intros E. eauto.
+    econstructor. eapply beq_nat_false_iff in E. omega.
+  - eapply closed_upgrade. eassumption. omega.
+Qed.
+
+Lemma indexr_has: forall X (G: list X) x,
+  length G > x ->
+  exists v, indexr x G = Some v.
+Proof.
+  intros. remember (length G) as n.
+  generalize dependent x.
+  generalize dependent G.
+  induction n; intros; try omega.
+  destruct G; simpl.
+  - simpl in Heqn. inversion Heqn.
+  - simpl in Heqn. inversion Heqn. subst.
+    case_eq (beq_nat x (length G)); intros E.
+    + eexists. reflexivity.
+    + apply beq_nat_false in E. apply IHn; eauto.
+      omega.
+Qed.
+
+Lemma stp_refl_aux: forall n T G GH,
+  closed 0 (length GH) (length G) T ->
+  tsize_flat T < n ->
+  stp G GH T T.
+Proof.
+  intros n. induction n; intros; try omega.
+  inversion H; subst; eauto;
+  try solve [omega];
+  try solve [simpl in H0; constructor; apply IHn; eauto; try omega];
+  try solve [apply indexr_has in H1; destruct H1; eauto].
+  - simpl in H0.
+    eapply stp_all.
+    eapply IHn; eauto; try omega.
+    reflexivity.
+    assumption.
+    assumption.
+    apply IHn; eauto.
+    simpl. apply closed_open; auto using closed_inc.
+    unfold open. rewrite <- open_preserves_size. omega.
+  - remember (open (varH (length GH)) T0) as TT.
+    assert (stp G (TT :: GH) TT TT). eapply IHn. subst.
+    eapply closed_open. simpl. eapply closed_upgrade_free. eassumption. omega.
+    constructor. simpl. omega. subst. unfold open. erewrite <- open_preserves_size. simpl in H0. omega.
+    eapply stp_bindx; try eassumption.
+  - simpl in *. assert (stp G GH T1 T1). eapply IHn; try eassumption; try omega.
+    assert (stp G GH T2 T2). eapply IHn; try eassumption; try omega.
+    eapply stp_and2; try eassumption. econstructor; try eassumption. eapply stp_and12; try eassumption.
+Qed.
+
+Lemma stp_refl: forall T G GH,
+  closed 0 (length GH) (length G) T ->
+  stp G GH T T.
+Proof.
+  intros. apply stp_refl_aux with (n:=S (tsize_flat T)); eauto.
+Qed.
+
+
+Lemma concat_same_length: forall {X} (GU: list X) (GL: list X) (GH1: list X) (GH0: list X),
+  GU ++ GL = GH1 ++ GH0 ->
+  length GU = length GH1 ->
+  GU=GH1 /\ GL=GH0.
+Proof.
+  intros. generalize dependent GH1. induction GU; intros.
+  - simpl in H0. induction GH1. rewrite app_nil_l in H. rewrite app_nil_l in H.
+    split. reflexivity. apply H.
+    simpl in H0. omega.
+  - simpl in H0. induction GH1. simpl in H0. omega.
+    simpl in H0. inversion H0. simpl in H. inversion H. specialize (IHGU GH1 H4 H2).
+    destruct IHGU. subst. split; reflexivity.
+Qed.
+
+Lemma concat_same_length': forall {X} (GU: list X) (GL: list X) (GH1: list X) (GH0: list X),
+  GU ++ GL = GH1 ++ GH0 ->
+  length GL = length GH0 ->
+  GU=GH1 /\ GL=GH0.
+Proof.
+  intros.
+  assert (length (GU ++ GL) = length (GH1 ++ GH0)) as A. {
+    rewrite H. reflexivity.
+  }
+  rewrite app_length in A. rewrite app_length in A.
+  rewrite H0 in A. apply Nat.add_cancel_r in A.
+  apply concat_same_length; assumption.
+Qed.
+
+
+Lemma indexr_at_index: forall {A} x0 GH0 GH1 (v:A),
+  beq_nat x0 (length GH1) = true ->
+  indexr x0 (GH0 ++ v :: GH1) = Some v.
+Proof.
+  intros. apply beq_nat_true in H. subst.
+  induction GH0.
+  - simpl. rewrite <- beq_nat_refl. reflexivity.
+  - simpl.
+    rewrite app_length. simpl. rewrite <- plus_n_Sm. rewrite <- plus_Sn_m.
+    rewrite false_beq_nat. assumption. omega.
+Qed.
+
+Lemma indexr_same: forall {A} x0 (v0:A) GH0 GH1 (v:A) (v':A),
+  beq_nat x0 (length GH1) = false ->
+  indexr x0 (GH0 ++ v :: GH1) = Some v0 ->
+  indexr x0 (GH0 ++ v' :: GH1) = Some v0.
+Proof.
+  intros ? ? ? ? ? ? ? E H.
+  induction GH0.
+  - simpl. rewrite E. simpl in H. rewrite E in H. apply H.
+  - simpl.
+    rewrite app_length. simpl.
+    case_eq (beq_nat x0 (length GH0 + S (length GH1))); intros E'.
+    simpl in H. rewrite app_length in H. simpl in H. rewrite E' in H.
+    rewrite H. reflexivity.
+    simpl in H. rewrite app_length in H. simpl in H. rewrite E' in H.
+    rewrite IHGH0. reflexivity. assumption.
+Qed.
+
+Inductive venv_ext : venv -> venv -> Prop :=
+| venv_ext_refl : forall G, venv_ext G G
+| venv_ext_cons : forall T G1 G2, venv_ext G1 G2 -> venv_ext (T::G1) G2.
+
+Lemma venv_ext__ge_length:
+  forall G G',
+    venv_ext G' G ->
+    length G' >= length G.
+Proof.
+  intros. induction H; simpl; omega.
+Qed.
+
+
+(* ### Substitution for relating static and dynamic semantics ### *)
+Lemma indexr_hit2 {X}: forall x (B:X) A G,
+  length G = x ->
+  B = A ->
+  indexr x (B::G) = Some A.
+Proof.
+  intros.
+  unfold indexr.
+  assert (beq_nat x (length G) = true). eapply beq_nat_true_iff. eauto.
+  rewrite H1. subst. reflexivity.
+Qed.
+
+Lemma indexr_miss {X}: forall x (B:X) A G,
+  indexr x (B::G) = A ->
+  x <> (length G)  ->
+  indexr x G = A.
+Proof.
+  intros.
+  unfold indexr in H.
+  assert (beq_nat x (length G) = false). eapply beq_nat_false_iff. eauto.
+  rewrite H1 in H. eauto.
+Qed.
+
+Lemma indexr_hit {X}: forall x (B:X) A G,
+  indexr x (B::G) = Some A ->
+  x = length G ->
+  B = A.
+Proof.
+  intros.
+  unfold indexr in H.
+  assert (beq_nat x (length G) = true). eapply beq_nat_true_iff. eauto.
+  rewrite H1 in H. inversion H. eauto.
+Qed.
+
+Lemma indexr_hit0: forall GH (GX0:venv) (TX0:ty),
+      indexr 0 (GH ++ [(GX0, TX0)]) =
+      Some (GX0, TX0).
+Proof.
+  intros GH. induction GH.
+  - intros. simpl. eauto.
+  - intros. simpl. destruct a. simpl. rewrite app_length. simpl.
+    assert (length GH + 1 = S (length GH)). omega. rewrite H.
+    eauto.
+Qed.
+
+Hint Resolve beq_nat_true_iff.
+Hint Resolve beq_nat_false_iff.
+
+Lemma closed_no_open: forall T x i j k,
+  closed i j k T ->
+  T = open_rec i x T.
+Proof.
+  intros. induction H; intros; eauto;
+  try solve [compute; compute in IHclosed; rewrite <-IHclosed; auto];
+  try solve [compute; compute in IHclosed1; compute in IHclosed2;
+             rewrite <-IHclosed1; rewrite <-IHclosed2; auto].
+
+  Case "TVarB".
+    unfold open_rec. assert (i <> x0). omega.
+    apply beq_nat_false_iff in H0.
+    rewrite H0. auto.
+Qed.
+
+Lemma open_subst_commute: forall T2 V j k x i,
+closed i j k (TSel V) ->
+(open_rec i (varH x) (subst V T2)) =
+(subst V (open_rec i (varH (x+1)) T2)).
+Proof.
+  intros T2 TX j k. induction T2; intros; eauto; try destruct v; eauto.
+  - simpl. rewrite IHT2_1; eauto. rewrite IHT2_2; eauto.
+    eapply closed_upgrade. eauto. eauto.
+  - simpl.
+    case_eq (beq_nat i 0); intros E.
+    apply beq_nat_true in E. subst.
+    case_eq (beq_nat i0 0); intros E0.
+    apply beq_nat_true in E0. subst.
+    destruct TX; eauto.
+    simpl. destruct i; eauto.
+    inversion H; subst. omega.
+    simpl. reflexivity.
+    case_eq (beq_nat i0 0); intros E0.
+    apply beq_nat_true in E0. subst.
+    simpl. destruct TX; eauto.
+    case_eq (beq_nat i i0); intros E1.
+    apply beq_nat_true in E1. subst.
+    inversion H; subst. omega.
+    reflexivity.
+    simpl. reflexivity.
+  - simpl.
+    case_eq (beq_nat i i0); intros E.
+    apply beq_nat_true in E; subst.
+    simpl.
+    assert (x+1 <> 0) as A by omega.
+    eapply beq_nat_false_iff in A.
+    rewrite A.
+    assert (x = x + 1 - 1) as B. unfold id. omega.
+    rewrite <- B. reflexivity.
+    simpl. reflexivity.
+  - simpl. rewrite IHT2_1. rewrite IHT2_2. eauto. eauto. eauto.
+  - simpl. rewrite IHT2. reflexivity. eapply closed_upgrade. eassumption. omega.
+  - simpl. rewrite IHT2_1. rewrite IHT2_2. reflexivity. assumption. assumption.
+Qed.
+
+Lemma closed_no_subst: forall T i k TX,
+   closed i 0 k T ->
+   subst TX T = T.
+Proof.
+  intros T. induction T; intros; inversion H; simpl; eauto;
+  try solve [rewrite (IHT i k TX); eauto; try omega];
+  try solve [rewrite (IHT1 i k TX); eauto; rewrite (IHT2 (S i) k TX); eauto; try omega];
+  try solve [rewrite (IHT1 i k TX); eauto; rewrite (IHT2 i k TX); eauto; try omega];
+  try omega.
+  erewrite IHT. reflexivity. eassumption.
+Qed.
+
+Lemma closed_subst: forall i j k V T, closed i (j+1) k T -> closed 0 j k (TSel V) -> closed i j k (subst V T).
+Proof.
+  intros. generalize dependent i.
+  induction T; intros; inversion H;
+  try econstructor;
+  try eapply IHT1; eauto; try eapply IHT2; eauto; try eapply IHT; eauto.
+
+  - Case "TVarH". simpl.
+    case_eq (beq_nat x 0); intros E.
+    eapply closed_upgrade. eapply closed_upgrade_free.
+    eauto. omega. eauto. omega.
+    econstructor. assert (x > 0). eapply beq_nat_false_iff in E. omega. omega.
+Qed.
+
+Lemma closed_nosubst: forall i j k V T, closed i (j+1) k T -> nosubst T -> closed i j k (subst V T).
+Proof.
+  intros. generalize dependent i.
+  induction T; intros; inversion H;
+  try econstructor;
+  try eapply IHT1; eauto; try eapply IHT2; eauto; try eapply IHT; eauto; subst;
+  try inversion H0; eauto.
+
+  - Case "TVarH". simpl. simpl in H0. unfold id in H0.
+    assert (beq_nat x 0 = false) as E. apply beq_nat_false_iff. assumption.
+    rewrite E.
+    eapply cl_selh. omega.
+Qed.
+
+Lemma subst_open_commute_m: forall i j k k' j' V T2, closed (i+1) (j+1) k T2 -> closed 0 j' k' (TSel V) ->
+    subst V (open_rec i (varH (j+1)) T2) = open_rec i (varH j) (subst V T2).
+Proof.
+  intros.
+  generalize dependent i. generalize dependent j.
+  induction T2; intros; inversion H; simpl; eauto; subst;
+  try rewrite IHT2_1;
+  try rewrite IHT2_2;
+  try rewrite IHT2; eauto.
+  - Case "TVarH". simpl. case_eq (beq_nat x 0); intros E.
+    eapply closed_no_open. eapply closed_upgrade. eauto. omega.
+    eauto.
+  - Case "TVarB". simpl. case_eq (beq_nat i x); intros E.
+    simpl. case_eq (beq_nat (j+1) 0); intros E2.
+    eapply beq_nat_true_iff in E2. omega.
+    subst. assert (j+1-1 = j) as A. omega. rewrite A. eauto.
+    eauto.
+Qed.
+
+Lemma subst_open_commute: forall i j k k' V T2, closed (i+1) (j+1) k T2 -> closed 0 0 k' (TSel V) ->
+    subst V (open_rec i (varH (j+1)) T2) = open_rec i (varH j) (subst V T2).
+Proof.
+  intros. eapply subst_open_commute_m; eauto.
+Qed.
+
+Lemma subst_open_zero: forall i i' k TX T2, closed i' 0 k T2 ->
+    subst TX (open_rec i (varH 0) T2) = open_rec i TX T2.
+Proof.
+  intros. generalize dependent i'. generalize dependent i.
+  induction T2; intros; inversion H; simpl; eauto;
+  try solve [rewrite (IHT2_1 _ i'); eauto;
+             rewrite (IHT2_2 _ (S i')); eauto;
+             rewrite (IHT2_2 _ (S i')); eauto];
+  try solve [rewrite (IHT2_1 _ i'); eauto;
+             rewrite (IHT2_2 _ i'); eauto].
+  subst.
+  case_eq (beq_nat x 0); intros E. omega. omega.
+  case_eq (beq_nat i x); intros E. eauto. eauto.
+  erewrite IHT2. reflexivity. eassumption.
+Qed.
+
+Lemma Forall2_length: forall A B f (G1:list A) (G2:list B),
+                        Forall2 f G1 G2 -> length G1 = length G2.
+Proof.
+  intros. induction H.
+  eauto.
+  simpl. eauto.
+Qed.
+
+Lemma nosubst_intro: forall i k T, closed i 0 k T -> nosubst T.
+Proof.
+  intros. generalize dependent i.
+  induction T; intros; inversion H; simpl; eauto.
+  omega.
+Qed.
+
+Lemma nosubst_open: forall i V T2, nosubst (TSel V) -> nosubst T2 -> nosubst (open_rec i V T2).
+Proof.
+  intros. generalize dependent i. induction T2; intros;
+  try inversion H0; simpl; eauto; destruct v; eauto.
+  case_eq (beq_nat i i0); intros E. eauto. eauto.
+Qed.
+
+
+Lemma indexr_hit_high: forall (X:Type) x (jj : X) l1 l2 vf,
+  indexr x (l1 ++ l2) = Some vf -> (length l2) <= x ->
+  indexr (x + 1) (l1 ++ jj :: l2) = Some vf.
+Proof. intros. induction l1. simpl in *. apply indexr_max in H. omega.
+  simpl in *. destruct (beq_nat x (length (l1 ++ l2))) eqn : A.
+  rewrite beq_nat_true_iff in A. assert (x + 1 = length (l1 ++ l2) + 1).
+  omega. rewrite app_length in *. assert(x + 1 = length (l1) + S (length l2)).
+  omega. simpl in *. rewrite <- beq_nat_true_iff in H2. rewrite H2. assumption.
+  rewrite beq_nat_false_iff in A. assert (x + 1 <> length (l1 ++ l2) + 1).
+  omega. rewrite app_length in *. assert(x + 1 <> length (l1) + S (length l2)). omega.
+  rewrite <- beq_nat_false_iff in H2. simpl. rewrite H2. apply IHl1. assumption.
+Qed.
+
+Lemma indexr_hit_low: forall (X:Type) x (jj : X) l1 l2 vf,
+  indexr x (l1 ++ l2) = Some vf -> x < (length l2) ->
+  indexr (x) (l1 ++ jj :: l2) = Some vf.
+Proof. intros. apply indexr_has in H0. ev. assert (indexr x (l1 ++ l2) = Some x0).
+  apply indexr_extend_mult. assumption. rewrite H1 in H. inversion H. subst.
+  assert (indexr x (jj :: l2) = Some vf). apply indexr_extend. assumption.
+  apply indexr_extend_mult. eassumption.
+Qed.
+
+Lemma splice_preserves_size: forall T j,
+  tsize_flat T = tsize_flat (splice j T).
+Proof.
+  intros. induction T; simpl; try rewrite IHT1; try rewrite IHT2; try reflexivity.
+  destruct v; simpl; try reflexivity. destruct (le_lt_dec j i); simpl; try reflexivity.
+  rewrite IHT. reflexivity.
+Qed.
+
+Lemma open_permute : forall T V0 V1 i j a b c d,
+  closed 0 a b (TSel V0) -> closed 0 c d (TSel V1) -> i <> j ->
+  open_rec i V0 (open_rec j V1 T) = open_rec j V1 (open_rec i V0 T).
+Proof. intros. generalize dependent i. generalize dependent j.
+  induction T; intros.
+  simpl. reflexivity.
+  simpl. reflexivity.
+  simpl. specialize (IHT1 _ _ H1). rewrite IHT1. assert ((S i) <> (S j)) by omega.
+  specialize (IHT2 _ _ H2). rewrite IHT2. reflexivity.
+  destruct v. simpl. reflexivity. simpl. reflexivity.
+  (* varB *)
+  destruct (beq_nat i i0) eqn : A. rewrite beq_nat_true_iff in A. subst.
+  assert ((open_rec j V1 (TSel (varB i0)) = (TSel (varB i0)))). simpl.
+  assert (beq_nat j i0 = false). rewrite beq_nat_false_iff. omega. rewrite H2. reflexivity.
+  rewrite H2. simpl. assert (beq_nat i0 i0 = true). erewrite beq_nat_refl. eauto. rewrite H3.
+  eapply closed_no_open. eapply closed_upgrade. eauto. omega.
+  destruct (beq_nat j i0) eqn : B. rewrite beq_nat_true_iff in B. subst.
+  simpl. assert (beq_nat i0 i0 = true). erewrite beq_nat_refl. eauto. rewrite H2.
+  assert (beq_nat i i0 = false). rewrite beq_nat_false_iff. omega. rewrite H3.
+  assert (TSel (V1) = open_rec i V0 (TSel V1)). eapply closed_no_open. eapply closed_upgrade.
+  eapply H0. omega. rewrite <- H4. simpl. rewrite H2. reflexivity.
+  assert ((open_rec j V1 (TSel (varB i0))) = TSel (varB i0)). simpl. rewrite B. reflexivity.
+  rewrite H2. assert (open_rec i V0 (TSel (varB i0)) = (TSel (varB i0))). simpl.
+  rewrite A. reflexivity. rewrite H3. simpl. rewrite B. reflexivity.
+
+  simpl. specialize (IHT1 _ _ H1). rewrite IHT1.
+  specialize (IHT2 _ _ H1). rewrite IHT2. reflexivity.
+  simpl. rewrite IHT. reflexivity. omega.
+  simpl. rewrite IHT1. rewrite IHT2. reflexivity. omega. omega.
+Qed.
+
+Lemma closed_open2: forall i j k V T i1, closed i j k T -> closed i j k (TSel V) ->
+  closed i j k (open_rec i1 V T).
+Proof.
+  intros. generalize dependent i. revert i1.
+  induction T; intros; inversion H;
+  try econstructor;
+  try eapply IHT1; eauto; try eapply IHT2; eauto; try eapply IHT; eauto.
+  eapply closed_upgrade. eauto. eauto.
+  - Case "TVarB". simpl.
+    case_eq (beq_nat i1 x); intros E. eauto.
+    econstructor. eapply beq_nat_false_iff in E. omega.
+  - eapply closed_upgrade. eassumption. omega.
+Qed.
+
+
+Lemma splice_retreat4: forall T i j k m V' V ,
+  closed i (j + 1) k (open_rec m V' (splice 0 T)) ->
+  (closed i j k (TSel V) -> closed i (j) k (open_rec m V T)).
+Proof. induction T; intros; try destruct v; simpl in *.
+  constructor.
+  constructor.
+  inversion H; subst.
+  specialize (IHT1 _ _ _ _ _ _ H6 H0). assert (closed (S i) (j) k (TSel V)).
+  eapply closed_upgrade. eapply H0. omega.
+  specialize (IHT2 _ _ _ _ _ _ H7 H1). constructor. assumption. assumption.
+  inversion H. subst. constructor. omega.
+  inversion H. subst. constructor. omega.
+  destruct (beq_nat m i0) eqn : A. assumption.
+    inversion H. subst. constructor. omega.
+  inversion H. subst. constructor. eapply IHT1. eassumption. assumption.
+  eapply IHT2. eassumption. assumption.
+  constructor. inversion H. subst.  eapply IHT; try eassumption. eapply closed_upgrade. eassumption. omega.
+  inversion H. subst. constructor.  eapply IHT1; try eassumption.
+  eapply IHT2; try eassumption.
+Qed.
+
+Lemma splice_retreat5: forall T i j k m V' V ,
+  closed i (j + 1) k (TSel V') -> closed i (j) k (open_rec m V T) ->
+  closed i (j + 1) k (open_rec m V' (splice 0 T)).
+Proof. induction T; intros; try destruct v; simpl in *.
+  constructor.
+  constructor.
+  inversion H0; subst.
+  specialize (IHT1 _ _ _ _ _ _ H H6). assert (closed (S i) (j + 1) k (TSel V')).
+  eapply closed_upgrade. eapply H. omega.
+  specialize (IHT2 _ _ _ _ _ _ H1 H7). constructor. assumption. assumption.
+  inversion H0. subst. constructor. omega.
+  inversion H0. subst. constructor. omega.
+  destruct (beq_nat m i0) eqn : A. assumption.
+    inversion H0. subst. constructor. omega.
+  inversion H0. subst. constructor. eapply IHT1. eassumption. eassumption.
+  eapply IHT2. eassumption. eassumption.
+  inversion H0. subst. constructor. eapply IHT; try eassumption. eapply closed_upgrade. eassumption. omega.
+  inversion H0. subst. constructor. eapply IHT1; try eassumption. eapply IHT2; try eassumption.
+
+Qed.
+
+
+
+Lemma splice_open_permute0: forall x0 T2 n j,
+(open_rec j (varH (n + x0 + 1 )) (splice (x0) T2)) =
+(splice (x0) (open_rec j (varH (n + x0)) T2)).
+Proof.
+  intros x0 T. induction T; intros; simpl; eauto;
+  try rewrite IHT1; try rewrite IHT2; try rewrite IHT; eauto;
+  destruct v; eauto.
+
+  case_eq (le_lt_dec (x0) i); intros E LE; simpl; eauto.
+  rewrite LE. eauto.
+  rewrite LE. eauto.
+  case_eq (beq_nat j i); intros E; simpl; eauto.
+  case_eq (le_lt_dec (x0) (n + x0)); intros EL LE.
+  rewrite E. eauto. omega.
+  rewrite E. eauto.
+Qed.
+
+Lemma indexr_extend_end: forall {X : Type} (jj : X) l x,
+  indexr (x + 1) (l ++ [jj]) = indexr x l.
+Proof. intros. induction l. simpl. assert (beq_nat (x + 1) 0 = false).
+  rewrite beq_nat_false_iff. omega. rewrite H. reflexivity.
+  simpl. destruct (beq_nat (x) (length (l))) eqn : A.
+  rewrite beq_nat_true_iff in A. assert (x + 1 = length (l ++ [jj])). rewrite app_length. simpl. omega.
+  rewrite <- beq_nat_true_iff in H. rewrite H. reflexivity.
+  rewrite beq_nat_false_iff in A. assert (x +1 <> length (l ++ [jj])). rewrite app_length. simpl. omega.
+  rewrite <- beq_nat_false_iff in H. rewrite H. assumption.
+Qed.
+
+Lemma indexr_hit01: forall {X : Type} GH (jj : X),
+      indexr 0 (GH ++ [jj]) = Some (jj).
+Proof.
+  intros X GH. induction GH.
+  - intros. simpl. eauto.
+  - intros. simpl. destruct (length (GH ++ [jj])) eqn : A.
+    rewrite app_length in *. simpl in *. omega.
+    apply IHGH.
+Qed.
+  
